starting adapting to word32

Weidenbach_Book/CDCL_Two_Watched_Literals_List_Watched_Code_Common.thy
@@ -1,8 +1,10 @@
 theory CDCL_Two_Watched_Literals_List_Watched_Code_Common
   imports CDCL_Two_Watched_Literals_Code_Common CDCL_Two_Watched_Literals_List_Watched_Domain
-    Bits_Natural
+    Bits_Natural WB_Word_Assn
 begin
 
+lemma \<open>(return o (\<lambda>n. shiftr n 1), RETURN o shiftr1) \<in> word_nat_assn\<^sup>k \<rightarrow>\<^sub>a word_nat_assn\<close>
+  by sepref_to_hoare (sep_auto simp: shiftr1_def word_nat_rel_def unat_shiftr br_def)
 
 section \<open>Code Generation\<close>
 
@@ -13,9 +15,9 @@ definition propagated where
 
 lemma propagated_hnr[sepref_fr_rules]:
   \<open>(uncurry (return oo propagated), uncurry (RETURN oo Propagated)) \<in>
-     nat_lit_assn\<^sup>k *\<^sub>a nat_assn\<^sup>k \<rightarrow>\<^sub>a pair_nat_ann_lit_assn\<close>
+     unat_lit_assn\<^sup>k *\<^sub>a nat_assn\<^sup>k \<rightarrow>\<^sub>a pair_nat_ann_lit_assn\<close>
   by sepref_to_hoare (sep_auto simp: nat_ann_lit_rel_def propagated_def case_prod_beta p2rel_def
-      lit_of_natP_def simp del: literal_of_nat.simps
+      lit_of_natP_def br_def uint32_nat_rel_def unat_lit_rel_def nat_lit_rel_def
       split: option.splits)
 
 definition decided where
@@ -23,46 +25,118 @@ definition decided where
 
 lemma decided_hnr[sepref_fr_rules]:
   \<open>(return o decided, RETURN o Decided) \<in>
-     nat_lit_assn\<^sup>k \<rightarrow>\<^sub>a pair_nat_ann_lit_assn\<close>
+     unat_lit_assn\<^sup>k \<rightarrow>\<^sub>a pair_nat_ann_lit_assn\<close>
   by sepref_to_hoare (sep_auto simp: nat_ann_lit_rel_def decided_def case_prod_beta p2rel_def
-      lit_of_natP_def simp del: literal_of_nat.simps
+      lit_of_natP_def br_def uint32_nat_rel_def unat_lit_rel_def nat_lit_rel_def
       split: option.splits)
 
 definition uminus_lit_imp :: \<open>nat \<Rightarrow> nat\<close> where
   \<open>uminus_lit_imp L = bitXOR L 1\<close>
 
-lemma uminus_lit_imp_hnr[sepref_fr_rules]:
-  \<open>(return o uminus_lit_imp, RETURN o uminus) \<in>
-     nat_lit_assn\<^sup>k \<rightarrow>\<^sub>a nat_lit_assn\<close>
+lemma nat_bin_trunc_ao:
+  \<open>nat (bintrunc n a) AND nat (bintrunc n b) = nat (bintrunc n (a AND b))\<close>
+  \<open>nat (bintrunc n a) OR nat (bintrunc n b) = nat (bintrunc n (a OR b))\<close>
+  unfolding bitAND_nat_def bitOR_nat_def
+  by (auto simp add: bin_trunc_ao bintr_ge0)
+
+lemma nat_uint_XOR: \<open>nat (uint (a XOR b)) = nat (uint a) XOR nat (uint b)\<close>
+  if len: \<open>LENGTH('a) > 0\<close>
+  for a b :: \<open>'a ::len0 Word.word\<close>
+proof -
+  have 1: \<open>uint ((word_of_int:: int \<Rightarrow> 'a Word.word)(uint a)) = uint a\<close>
+    by (subst (2) word_of_int_uint[of a, symmetric]) (rule refl)
+  have H: \<open>nat (bintrunc n (a XOR b)) = nat (bintrunc n a XOR bintrunc n b)\<close>
+    if \<open>n> 0\<close> for n and a :: int and b :: int
+    using that
+    apply (induction n arbitrary: a b)
+    subgoal by auto
+    subgoal for n a b
+      apply (cases n)
+       apply (auto simp: bintr_ge0) -- \<open>TODO tune proof\<close>
+      by (smt BIT_lt0 bintr_ge0 int_nat_eq int_xor_lt0)
+    done
+  have \<open>nat (bintrunc LENGTH('a) (a XOR b)) = nat (bintrunc LENGTH('a) a XOR bintrunc LENGTH('a) b)\<close> for a b
+    using len H[of \<open>LENGTH('a)\<close> a b] by (auto simp: bintrunc_minus_simps)
+  then have \<open>nat (uint (a XOR b)) = nat (uint a XOR uint b)\<close>
+    by transfer
+  then show ?thesis
+    unfolding bitXOR_nat_def by auto
+qed
+
+lemma nat_of_uint32_XOR: \<open>nat_of_uint32 (a XOR b) = nat_of_uint32 a XOR nat_of_uint32 b\<close>
+  by transfer (auto simp: unat_def nat_uint_XOR)
+
+lemma uminus_lit_imp_uminus:
+  \<open>(RETURN o uminus_lit_imp, RETURN o uminus) \<in>
+     nat_lit_rel \<rightarrow>\<^sub>f \<langle>nat_lit_rel\<rangle>nres_rel\<close>
   unfolding bitXOR_1_if_mod_2 uminus_lit_imp_def
-  apply sepref_to_hoare
-  apply (sep_auto simp: nat_ann_lit_rel_def uminus_lit_imp_def case_prod_beta p2rel_def
-      lit_of_natP_def split: option.splits)
-  by presburger
+  by (intro frefI nres_relI) (auto simp: nat_ann_lit_rel_def uminus_lit_imp_def case_prod_beta p2rel_def
+      lit_of_natP_def nat_lit_rel_def split: option.splits, presburger)
+
+lemma bitXOR_uminus[sepref_fr_rules]:
+  \<open>(return o (\<lambda>L. bitXOR L 1), RETURN o uminus) \<in>
+     unat_lit_assn\<^sup>k \<rightarrow>\<^sub>a unat_lit_assn\<close>
+proof -
+  have [simp]: \<open>nat_of_uint32 1 = 1\<close>
+    by transfer auto
+  have [simp]: \<open>0 XOR Suc 0 = Suc 0\<close>
+    unfolding bitXOR_nat_def
+    by auto
+  have [simp]: \<open>bin_last (2 + n) = bin_last n\<close> for n
+    by (auto simp: bin_last_def)
+  have [simp]: \<open>bin_rest (2 + n) = 1 + (bin_rest n)\<close> for n
+    by (auto simp: bin_rest_def)
+  have \<open>bin_nth (2 + n XOR 1) na \<longleftrightarrow> bin_nth (2 + (n XOR 1)) na\<close> for n na
+    by (induction na)  auto
+
+  then have [simp]: \<open>((2 + n) XOR 1) = 2 + ( ( ( n XOR 1)))\<close> for n :: int
+    by (auto simp: bin_eq_iff)
+
+  have [simp]: \<open>Suc (Suc n) XOR Suc 0 = Suc (Suc (n XOR Suc 0))\<close> for n :: nat
+    unfolding bitXOR_nat_def
+    by (auto simp: nat_add_distrib)
+
+  have [simp]: \<open>2 * q XOR Suc 0 = Suc (2 * q)\<close> for q :: nat
+    by (induction q)  auto
+
+  have 1: \<open>(return o (\<lambda>L. bitXOR L 1), RETURN o uminus_lit_imp) \<in>
+     uint32_nat_assn\<^sup>k \<rightarrow>\<^sub>a uint32_nat_assn\<close>
+    unfolding bitXOR_1_if_mod_2 uminus_lit_imp_def
+    apply sepref_to_hoare
+    apply (sep_auto simp: nat_ann_lit_rel_def uminus_lit_imp_def case_prod_beta p2rel_def
+        lit_of_natP_def uint32_nat_rel_def br_def nat_of_uint32_XOR bitXOR_1_if_mod_2
+        split: option.splits)
+    using One_nat_def bitXOR_1_if_mod_2 by presburger
+  show ?thesis
+    using 1[FCOMP uminus_lit_imp_uminus] unfolding unat_lit_rel_def .
+qed
 
 
 subsection \<open>State Conversion\<close>
 
 subsubsection \<open>Functions and Types:\<close>
- 
-type_synonym clauses_wl = \<open>nat arrayO_raa\<close>
+
+type_synonym clauses_wl = \<open>uint32 arrayO_raa\<close>
+
+abbreviation uint32_assn :: \<open>uint32 \<Rightarrow> uint32 \<Rightarrow> assn\<close> where
+  \<open>uint32_assn \<equiv> id_assn\<close>
 
 abbreviation ann_lit_wl_assn :: \<open>ann_lit_wl \<Rightarrow> ann_lit_wl \<Rightarrow> assn\<close> where
-  \<open>ann_lit_wl_assn \<equiv> prod_assn nat_assn (option_assn nat_assn)\<close>
+  \<open>ann_lit_wl_assn \<equiv> prod_assn uint32_assn (option_assn nat_assn)\<close>
 
 abbreviation ann_lits_wl_assn :: \<open>ann_lits_wl \<Rightarrow> ann_lits_wl \<Rightarrow> assn\<close> where
   \<open>ann_lits_wl_assn \<equiv> list_assn ann_lit_wl_assn\<close>
 
 abbreviation clause_ll_assn :: "nat clause_l \<Rightarrow> clause_wl \<Rightarrow> assn" where
-  \<open>clause_ll_assn \<equiv> array_assn nat_lit_assn\<close>
+  \<open>clause_ll_assn \<equiv> array_assn unat_lit_assn\<close>
 
 abbreviation clauses_ll_assn :: "nat clauses_l \<Rightarrow> clauses_wl \<Rightarrow> assn" where
-  \<open>clauses_ll_assn \<equiv> arlO_assn (array_assn nat_lit_assn)\<close>
+  \<open>clauses_ll_assn \<equiv> arlO_assn clause_ll_assn\<close>
 
-abbreviation clause_l_assn :: "nat clause \<Rightarrow> nat list \<Rightarrow> assn" where
-  \<open>clause_l_assn \<equiv> list_mset_assn nat_lit_assn\<close>
+abbreviation clause_l_assn :: "nat clause \<Rightarrow> uint32 list \<Rightarrow> assn" where
+  \<open>clause_l_assn \<equiv> list_mset_assn unat_lit_assn\<close>
 
-abbreviation clauses_l_assn :: "nat clauses \<Rightarrow> nat list list \<Rightarrow> assn" where
+abbreviation clauses_l_assn :: "nat clauses \<Rightarrow> uint32 list list \<Rightarrow> assn" where
   \<open>clauses_l_assn \<equiv> list_mset_assn clause_l_assn\<close>
 
 abbreviation clauses_to_update_l_assn :: "nat multiset \<Rightarrow> nat list \<Rightarrow> assn" where
@@ -72,18 +146,18 @@ abbreviation clauses_to_update_ll_assn :: "nat list \<Rightarrow> nat list \<Rig
   \<open>clauses_to_update_ll_assn \<equiv> list_assn nat_assn\<close>
 
 abbreviation unit_lits_assn :: "nat clauses \<Rightarrow> unit_lits_wl \<Rightarrow> assn" where
-  \<open>unit_lits_assn \<equiv> list_mset_assn (list_mset_assn nat_lit_assn)\<close>
+  \<open>unit_lits_assn \<equiv> list_mset_assn (list_mset_assn unat_lit_assn)\<close>
 
-abbreviation conflict_assn :: "nat clause \<Rightarrow> nat array_list \<Rightarrow> assn" where
-  \<open>conflict_assn \<equiv> hr_comp (arl_assn nat_lit_assn) list_mset_rel\<close>
+abbreviation conflict_assn :: "nat clause \<Rightarrow> uint32 array_list \<Rightarrow> assn" where
+  \<open>conflict_assn \<equiv> hr_comp (arl_assn unat_lit_assn) list_mset_rel\<close>
 
-abbreviation conflict_option_assn :: "nat clause option \<Rightarrow> nat array_list option \<Rightarrow> assn" where
+abbreviation conflict_option_assn :: "nat clause option \<Rightarrow> uint32 array_list option \<Rightarrow> assn" where
   \<open>conflict_option_assn \<equiv> option_assn conflict_assn\<close>
 
 type_synonym nat_clauses_l = \<open>nat list list\<close>
 
 type_synonym twl_st_wll =
-  "nat_trail \<times> clauses_wl \<times> nat \<times> nat array_list option \<times>  unit_lits_wl \<times> unit_lits_wl \<times>
+  "nat_trail \<times> clauses_wl \<times> nat \<times> uint32 array_list option \<times>  unit_lits_wl \<times> unit_lits_wl \<times>
     lit_queue_l \<times> watched_wl"
 
 
@@ -143,17 +217,24 @@ lemma valued_impl_spec:
   unfolding fref_def nres_rel_def
   by (auto simp: valued_impl_valued IS_ID_def)
 
+lemma nat_of_uint32_shiftr: \<open>nat_of_uint32 (shiftr xi n) = (shiftr (nat_of_uint32 xi) n)\<close>
+  by transfer (auto simp: shiftr_div_2n unat_def shiftr_nat_def)
+
+
 lemma atm_of_hnr[sepref_fr_rules]:
-  \<open>(return o shiftr1, RETURN o op_atm_of) \<in> (pure nat_lit_rel)\<^sup>k \<rightarrow>\<^sub>a id_assn\<close>
-  by sepref_to_hoare (sep_auto simp: p2rel_def lit_of_natP_def shiftr1_def)
+  \<open>(return o (\<lambda>L. shiftr L 1), RETURN o op_atm_of) \<in> (pure unat_lit_rel)\<^sup>k \<rightarrow>\<^sub>a uint32_nat_assn\<close>
+  by sepref_to_hoare (sep_auto simp: p2rel_def lit_of_natP_def uint32_nat_rel_def br_def
+      Collect_eq_comp unat_lit_rel_def nat_of_uint32_shiftr nat_lit_rel_def)
 
 lemma lit_of_hnr[sepref_fr_rules]:
-  \<open>(return o fst, RETURN o op_lit_of) \<in> (pure nat_ann_lit_rel)\<^sup>k \<rightarrow>\<^sub>a (pure nat_lit_rel)\<close>
+  \<open>(return o fst, RETURN o op_lit_of) \<in> (pure nat_ann_lit_rel)\<^sup>k \<rightarrow>\<^sub>a (pure unat_lit_rel)\<close>
   apply sepref_to_hoare
-  apply (sep_auto simp: p2rel_def nat_ann_lit_rel_def lit_of_natP_def
+  apply (sep_auto simp: p2rel_def nat_ann_lit_rel_def lit_of_natP_def uint32_nat_rel_def
+      Collect_eq_comp br_def unat_lit_rel_def nat_lit_rel_def
       split: if_splits)
+  unfolding br_def
    apply (case_tac b)
-    apply auto[2]
+    apply simp_all
   apply (case_tac b)
    apply (auto
       elim!: run_elims
@@ -162,24 +243,32 @@ lemma lit_of_hnr[sepref_fr_rules]:
 
 lemma op_eq_op_nat_lit_eq[sepref_fr_rules]:
   \<open>(uncurry (return oo (op =)), uncurry (RETURN oo op_nat_lit_eq)) \<in>
-    (pure nat_lit_rel)\<^sup>k *\<^sub>a (pure nat_lit_rel)\<^sup>k \<rightarrow>\<^sub>a bool_assn\<close>
+    (pure unat_lit_rel)\<^sup>k *\<^sub>a (pure unat_lit_rel)\<^sup>k \<rightarrow>\<^sub>a bool_assn\<close>
 proof -
   have [simp]: \<open>even bi \<Longrightarrow> even ai \<Longrightarrow> ai div 2 = bi div 2 \<Longrightarrow> ai = bi\<close> for ai bi :: nat
     by presburger
   have [simp]: \<open>odd bi \<Longrightarrow> odd ai \<Longrightarrow> ai div 2 = bi div 2 \<Longrightarrow> ai = bi\<close> for ai bi :: nat
     by presburger
   show ?thesis
-    by sepref_to_hoare (sep_auto simp: p2rel_def nat_ann_lit_rel_def lit_of_natP_def
-      split: if_splits)
+    apply sepref_to_hoare
+    apply (sep_auto simp: p2rel_def nat_ann_lit_rel_def lit_of_natP_def nat_lit_rel_def
+        br_def Collect_eq_comp uint32_nat_rel_def dvd_div_eq_iff unat_lit_rel_def
+      split: if_splits)+
+    using \<open>\<And>bi ai. \<lbrakk>odd bi; odd ai; ai div 2 = bi div 2\<rbrakk> \<Longrightarrow> ai = bi\<close>
+      word_nat_of_uint32_Rep_inject by blast
 qed
 
+text \<open>TODO Move to declaration\<close>
+declare op_eq_uint32_nat[sepref_fr_rules]
+
+
 sepref_definition valued_impl' is \<open>uncurry valued_impl\<close>
-  :: \<open>pair_nat_ann_lits_assn\<^sup>k *\<^sub>a nat_lit_assn\<^sup>k \<rightarrow>\<^sub>a option_assn bool_assn\<close>
+  :: \<open>pair_nat_ann_lits_assn\<^sup>k *\<^sub>a unat_lit_assn\<^sup>k \<rightarrow>\<^sub>a option_assn bool_assn\<close>
   unfolding valued_impl_def Let_def
   by sepref
 
 lemma valued_impl'[sepref_fr_rules]: \<open>(uncurry valued_impl', uncurry (RETURN oo valued)) \<in>
-   [\<lambda>(a, b). no_dup a]\<^sub>a pair_nat_ann_lits_assn\<^sup>k *\<^sub>a (pure nat_lit_rel)\<^sup>k \<rightarrow> option_assn bool_assn\<close>
+   [\<lambda>(a, b). no_dup a]\<^sub>a pair_nat_ann_lits_assn\<^sup>k *\<^sub>a unat_lit_assn\<^sup>k \<rightarrow> option_assn bool_assn\<close>
   using valued_impl'.refine[FCOMP valued_impl_spec] by auto
 
 definition delete_index_and_swap_ll where
@@ -242,7 +331,7 @@ subsection \<open>Code Generation\<close>
 
 subsubsection \<open>More Operations\<close>
 
-fun literals_to_update_wll :: \<open>twl_st_wll \<Rightarrow> nat list\<close> where
+fun literals_to_update_wll :: \<open>twl_st_wll \<Rightarrow> lit_queue_l\<close> where
   \<open>literals_to_update_wll (M, N, U, D, NP, UP, Q, W) = Q\<close>
 
 definition literals_to_update_wll_empty :: \<open>twl_st_wll \<Rightarrow> bool\<close> where
@@ -251,13 +340,27 @@ definition literals_to_update_wll_empty :: \<open>twl_st_wll \<Rightarrow> bool\
 definition literals_to_update_wl_empty :: \<open>nat twl_st_wl \<Rightarrow> bool\<close>  where
   \<open>literals_to_update_wl_empty = (\<lambda>(M, N, U, D, NP, UP, Q, W). Q = {#})\<close>
 
-definition select_and_remove_from_literals_to_update_wl' :: \<open>twl_st_wll \<Rightarrow> twl_st_wll \<times> nat\<close> where
+definition select_and_remove_from_literals_to_update_wl' :: \<open>twl_st_wll \<Rightarrow> twl_st_wll \<times> uint32\<close> where
   \<open>select_and_remove_from_literals_to_update_wl' =
     (\<lambda>(M, N, U, D, NP, UP, Q, W).  ((M, N, U, D, NP, UP, tl Q, W), hd Q))\<close>
 
+lemma nat_lit_eq[sepref_fr_rules]: \<open>(uncurry (return oo op =), uncurry (RETURN oo op =)) \<in>
+   (nat_lit_assn)\<^sup>k *\<^sub>a (nat_lit_assn)\<^sup>k \<rightarrow>\<^sub>a bool_assn\<close>
+  by sepref_to_hoare (sep_auto simp: p2rel_def nat_lit_rel_def
+      dest: lit_of_natP_same_rightD lit_of_natP_same_leftD)
+
+lemma unat_lit_eq[sepref_fr_rules]: \<open>(uncurry (return oo op =), uncurry (RETURN oo op =)) \<in>
+   (unat_lit_assn)\<^sup>k *\<^sub>a (unat_lit_assn)\<^sup>k \<rightarrow>\<^sub>a bool_assn\<close>
+  by sepref_to_hoare (sep_auto simp: p2rel_def unat_lit_rel_def
+      uint32_nat_rel_def br_def nat_lit_rel_def
+      dest: lit_of_natP_same_rightD lit_of_natP_same_leftD)
+
+text \<open>TODO Move declaration to definition\<close>
+declare op_eq_uint32_nat [sepref_fr_rules]
+
 sepref_thm list_contains_WHILE_array
   is \<open>uncurry (\<lambda>(l::nat) xs. do{ b \<leftarrow> list_contains_WHILE l xs; RETURN (fst b)})\<close>
-  :: \<open>nat_assn\<^sup>k *\<^sub>a (array_assn id_assn)\<^sup>k \<rightarrow>\<^sub>a bool_assn\<close>
+  :: \<open>uint32_nat_assn\<^sup>k *\<^sub>a (array_assn uint32_nat_assn)\<^sup>k \<rightarrow>\<^sub>a bool_assn\<close>
   unfolding list_contains_WHILE_def
   by sepref
 
@@ -281,7 +384,6 @@ proof -
         op_list_contains, unfolded conc_fun_chain]
     by simp
 qed
-
 
 definition list_contains_WHILE_f where
   \<open>list_contains_WHILE_f l xs = do{ b \<leftarrow> list_contains_WHILE l xs; RETURN (fst b)}\<close>
@@ -312,7 +414,7 @@ lemma in_nat_list_rel_list_all2_in_set_iff:
     apply (rotate_tac 2)
     apply (induction b ba rule: list_induct2)
      apply (solves simp)
-    apply (auto simp: p2rel_def lit_of_natP_same_leftD lit_of_natP_same_rightD)[]
+    apply (auto simp: p2rel_def lit_of_natP_same_leftD lit_of_natP_same_rightD nat_lit_rel_def)[]
     done
   subgoal using list_all2_lengthD by auto
   done
@@ -320,20 +422,20 @@ lemma in_nat_list_rel_list_all2_in_set_iff:
 lemma list_contains_WHILE_code_op_list_contains[sepref_fr_rules]:
   \<open>(uncurry list_contains_WHILE_array_code,
     uncurry (RETURN oo op_list_contains)) \<in>
-    nat_lit_assn\<^sup>k *\<^sub>a (clause_ll_assn)\<^sup>k \<rightarrow>\<^sub>a bool_assn\<close>
+    unat_lit_assn\<^sup>k *\<^sub>a (clause_ll_assn)\<^sup>k \<rightarrow>\<^sub>a bool_assn\<close>
 proof -
   have 1: \<open>(uncurry (RETURN oo op_list_contains), uncurry (RETURN oo op_list_contains)) \<in>
          nat_lit_rel \<times>\<^sub>r \<langle>nat_lit_rel\<rangle>list_rel \<rightarrow>\<^sub>f \<langle>bool_rel\<rangle>nres_rel\<close>
     by (intro frefI nres_relI) (auto simp: list_rel_def in_nat_list_rel_list_all2_in_set_iff)
   term nat_lit_rel
-  have 2: \<open>hr_comp (hr_comp (array_assn nat_assn) (\<langle>nat_rel\<rangle>list_rel))
-       (\<langle>nat_lit_rel\<rangle>list_rel) = array_assn nat_lit_assn\<close>
-    by (simp add: array_assn_def)
+  have 2: \<open>hr_comp (hr_comp (array_assn uint32_nat_assn) (\<langle>nat_rel\<rangle>list_rel))
+       (\<langle>nat_lit_rel\<rangle>list_rel) = array_assn unat_lit_assn\<close>
+    by (simp add: array_assn_def unat_lit_rel_def hr_comp_assoc list_rel_compp)
 
   show ?thesis
     using list_contains_WHILE_array_code.refine[unfolded list_contains_WHILE_f_def[symmetric],
         FCOMP list_contains_WHILE_f_op_list_contains, FCOMP 1]
-    unfolding 2 .
+    unfolding 2 unfolding unat_lit_rel_def .
 qed
 
 definition get_level_wl where
@@ -408,9 +510,10 @@ proof -
     unfolding 1 .
 qed
 
+text \<open>TODO: as levels are less than the numbers of literals, change to \<^typ>\<open>uint32\<close>?\<close>
 sepref_definition get_level_wl_code
   is \<open>uncurry (RETURN oo get_level_wl)\<close>
-  :: \<open>pair_nat_ann_lits_assn\<^sup>k *\<^sub>a nat_lit_assn\<^sup>k \<rightarrow>\<^sub>a nat_assn\<close>
+  :: \<open>pair_nat_ann_lits_assn\<^sup>k *\<^sub>a unat_lit_assn\<^sup>k \<rightarrow>\<^sub>a nat_assn\<close>
   unfolding get_level_wl_def[abs_def]
   by sepref
 
@@ -424,12 +527,12 @@ definition maximum_level_remove where
 
 lemma get_level_wl_code_get_level[sepref_fr_rules]:
   \<open>(uncurry get_level_wl_code, uncurry (RETURN oo (get_level :: (nat, nat) ann_lits \<Rightarrow> nat literal \<Rightarrow> nat))) \<in>
-    pair_nat_ann_lits_assn\<^sup>k *\<^sub>a nat_lit_assn\<^sup>k \<rightarrow>\<^sub>a nat_assn\<close>
+    pair_nat_ann_lits_assn\<^sup>k *\<^sub>a unat_lit_assn\<^sup>k \<rightarrow>\<^sub>a nat_assn\<close>
   using get_level_wl_code.refine unfolding get_level_wl_get_level[abs_def] .
 
 sepref_definition maximum_level_remove_code
   is \<open>uncurry2 (RETURN ooo maximum_level_remove)\<close>
-  :: \<open>pair_nat_ann_lits_assn\<^sup>k *\<^sub>a (arl_assn nat_lit_assn)\<^sup>k *\<^sub>a nat_lit_assn\<^sup>k \<rightarrow>\<^sub>a nat_assn\<close>
+  :: \<open>pair_nat_ann_lits_assn\<^sup>k *\<^sub>a (arl_assn unat_lit_assn)\<^sup>k *\<^sub>a unat_lit_assn\<^sup>k \<rightarrow>\<^sub>a nat_assn\<close>
   unfolding maximum_level_remove_def[abs_def]
   by sepref
 
@@ -470,7 +573,7 @@ definition get_maximum_level_remove where
 lemma maximum_level_remove_code_get_maximum_level_remove[sepref_fr_rules]:
   \<open>(uncurry2 (maximum_level_remove_code),
      uncurry2 (RETURN ooo get_maximum_level_remove)) \<in>
-    pair_nat_ann_lits_assn\<^sup>k *\<^sub>a conflict_assn\<^sup>k *\<^sub>a nat_lit_assn\<^sup>k \<rightarrow>\<^sub>a nat_assn\<close>
+    pair_nat_ann_lits_assn\<^sup>k *\<^sub>a conflict_assn\<^sup>k *\<^sub>a unat_lit_assn\<^sup>k \<rightarrow>\<^sub>a nat_assn\<close>
 proof -
   have 1:
   \<open>(uncurry2 (RETURN ooo maximum_level_remove),
@@ -616,30 +719,27 @@ lemma
     \<open>CONSTRAINT (IS_PURE IS_RIGHT_UNIQUE) nat_lit_assn\<close> and
   nat_lit_assn_left_unique:
     \<open>CONSTRAINT (IS_PURE IS_LEFT_UNIQUE) nat_lit_assn\<close>
-   by (auto simp: IS_PURE_def single_valued_def p2rel_def IS_LEFT_UNIQUE_def
+   by (auto simp: IS_PURE_def single_valued_def p2rel_def IS_LEFT_UNIQUE_def nat_lit_rel_def
       dest: lit_of_natP_same_rightD lit_of_natP_same_leftD)
 
-lemma nat_lit_eq[sepref_fr_rules]: \<open>(uncurry (return oo op =), uncurry (RETURN oo op =)) \<in>
-   (pure nat_lit_rel)\<^sup>k *\<^sub>a (pure nat_lit_rel)\<^sup>k \<rightarrow>\<^sub>a bool_assn\<close>
-  by sepref_to_hoare (sep_auto simp: p2rel_def dest: lit_of_natP_same_rightD lit_of_natP_same_leftD)
 
 sepref_definition is_in_arl_code
   is \<open>uncurry is_in_arl\<close>
-  :: \<open>(pure nat_lit_rel)\<^sup>k *\<^sub>a (arl_assn (pure nat_lit_rel))\<^sup>k \<rightarrow>\<^sub>a bool_assn\<close>
+  :: \<open>(pure unat_lit_rel)\<^sup>k *\<^sub>a (arl_assn (unat_lit_assn))\<^sup>k \<rightarrow>\<^sub>a bool_assn\<close>
   unfolding is_in_arl_def find_first_eq_def short_circuit_conv
   supply [[goals_limit = 1]]
   by sepref
 
 lemma is_in_arl_op_mset_contains_nat_lit_rel[sepref_fr_rules]:
   shows \<open>(uncurry is_in_arl_code, uncurry (RETURN oo op_mset_contains)) \<in>
-   (pure nat_lit_rel)\<^sup>k *\<^sub>a conflict_assn\<^sup>k \<rightarrow>\<^sub>a bool_assn\<close>
+   (pure unat_lit_rel)\<^sup>k *\<^sub>a conflict_assn\<^sup>k \<rightarrow>\<^sub>a bool_assn\<close>
 proof -
   have 1: \<open>IS_LEFT_UNIQUE Id\<close>
     using IS_LEFT_UNIQUE_def single_valued_def by auto
   have 2: \<open>list_mset_rel O \<langle>Id\<rangle>mset_rel = list_mset_rel\<close>
     by (auto simp add: list_mset_rel_def mset_rel_def br_def Collect_eq_comp rel2p_def[abs_def]
         p2rel_def rel_mset_def list.rel_eq)
-  have 3: \<open>(hr_comp (arl_assn nat_lit_assn) (list_mset_rel O \<langle>Id\<rangle>mset_rel)) = conflict_assn\<close>
+  have 3: \<open>(hr_comp (arl_assn unat_lit_assn) (list_mset_rel O \<langle>Id\<rangle>mset_rel)) = conflict_assn\<close>
     by (auto simp: hr_comp_def[abs_def] 2)
   show ?thesis
     using is_in_arl_code.refine[FCOMP is_in_arl_op_mset_contains, of Id]
@@ -663,7 +763,7 @@ definition remove1_wl where
 
 sepref_definition find_first_eq_code
   is \<open>uncurry find_first_eq\<close>
-  :: \<open>nat_assn\<^sup>k *\<^sub>a (arl_assn nat_assn)\<^sup>k \<rightarrow>\<^sub>a nat_assn\<close>
+  :: \<open>uint32_nat_assn\<^sup>k *\<^sub>a (arl_assn uint32_nat_assn)\<^sup>k \<rightarrow>\<^sub>a nat_assn\<close>
   unfolding find_first_eq_def short_circuit_conv
   by sepref
 
@@ -671,7 +771,7 @@ declare find_first_eq_code.refine[sepref_fr_rules]
 
 sepref_definition remove1_wl_code
   is \<open>uncurry remove1_wl\<close>
-  :: \<open>nat_assn\<^sup>k *\<^sub>a (arl_assn nat_assn)\<^sup>d \<rightarrow>\<^sub>a arl_assn nat_assn\<close>
+  :: \<open>uint32_nat_assn\<^sup>k *\<^sub>a (arl_assn uint32_nat_assn)\<^sup>d \<rightarrow>\<^sub>a arl_assn uint32_nat_assn\<close>
   unfolding remove1_wl_def short_circuit_conv
   by sepref
 
@@ -759,81 +859,84 @@ lemma remove1_remove1_mset: \<open>(uncurry (RETURN oo remove1), uncurry (RETURN
   apply (intro frefI nres_relI)
   using list_all2_remove
   by (fastforce simp: remove1_wl_def list_mset_rel_def br_def mset_rel_def p2rel_def
-      rel2p_def[abs_def] rel_mset_def Collect_eq_comp)
+      rel2p_def[abs_def] rel_mset_def Collect_eq_comp nat_lit_rel_def)
 
+
+lemma list_all2_op_eq_map_right_iff': \<open>list_all2 (\<lambda>L L'. L' = (f L)) a aa \<longleftrightarrow> aa = map f a \<close>
+  apply (induction a arbitrary: aa)
+   apply (auto; fail)
+  by (rename_tac aa, case_tac aa) (auto)
+
+lemma ex_assn_def_pure_eq_middle3:
+  \<open>(\<exists>\<^sub>Aba b bb. f b ba bb * \<up> (ba = h b bb) * P b ba bb) = (\<exists>\<^sub>Ab bb. f b (h b bb) bb * P b (h b bb) bb)\<close>
+  \<open>(\<exists>\<^sub>Ab ba bb. f b ba bb * \<up> (ba = h b bb) * P b ba bb) = (\<exists>\<^sub>Ab bb. f b (h b bb) bb * P b (h b bb) bb)\<close>
+  \<open>(\<exists>\<^sub>Ab bb ba. f b ba bb * \<up> (ba = h b bb) * P b ba bb) = (\<exists>\<^sub>Ab bb. f b (h b bb) bb * P b (h b bb) bb)\<close>
+  \<open>(\<exists>\<^sub>Aba b bb. f b ba bb * \<up> (ba = h b bb \<and> Q b ba bb)) = (\<exists>\<^sub>Ab bb. f b (h b bb) bb * \<up>(Q b (h b bb) bb))\<close>
+  \<open>(\<exists>\<^sub>Ab ba bb. f b ba bb * \<up> (ba = h b bb \<and> Q b ba bb)) = (\<exists>\<^sub>Ab bb. f b (h b bb) bb * \<up>(Q b (h b bb) bb))\<close>
+  \<open>(\<exists>\<^sub>Ab bb ba. f b ba bb * \<up> (ba = h b bb \<and> Q b ba bb)) = (\<exists>\<^sub>Ab bb. f b (h b bb) bb * \<up>(Q b (h b bb) bb))\<close>
+  by (subst ex_assn_def, subst (3) ex_assn_def, auto)+
+
+lemma ex_assn_def_pure_eq_middle2:
+  \<open>(\<exists>\<^sub>Aba b. f b ba  * \<up> (ba = h b) * P b ba) = (\<exists>\<^sub>Ab . f b (h b) * P b (h b))\<close>
+  \<open>(\<exists>\<^sub>Ab ba. f b ba  * \<up> (ba = h b) * P b ba) = (\<exists>\<^sub>Ab . f b (h b) * P b (h b))\<close>
+  \<open>(\<exists>\<^sub>Ab ba. f b ba  * \<up> (ba = h b \<and> Q b ba)) = (\<exists>\<^sub>Ab. f b (h b) * \<up>(Q b (h b)))\<close>
+  \<open>(\<exists>\<^sub>A ba b. f b ba  * \<up> (ba = h b \<and> Q b ba)) = (\<exists>\<^sub>Ab. f b (h b) * \<up>(Q b (h b)))\<close>
+  by (subst ex_assn_def, subst (2) ex_assn_def, auto)+
+
+lemma ex_assn_skip_first2:
+  \<open>(\<exists>\<^sub>Aba bb. f bb * \<up>(P ba bb)) = (\<exists>\<^sub>Abb. f bb * \<up>(\<exists>ba. P ba bb))\<close>
+  \<open>(\<exists>\<^sub>Abb ba. f bb * \<up>(P ba bb)) = (\<exists>\<^sub>Abb. f bb * \<up>(\<exists>ba. P ba bb))\<close>
+  apply (subst ex_assn_swap)
+  by (subst ex_assn_def, subst (2) ex_assn_def, auto)+
 
 lemma remove1_wl_code_op_mset_delete[sepref_fr_rules]:
   \<open>(uncurry (remove1_wl_code), uncurry (RETURN oo op_mset_delete)) \<in>
-     nat_lit_assn\<^sup>k *\<^sub>a conflict_assn\<^sup>d \<rightarrow>\<^sub>a conflict_assn\<close>
+     unat_lit_assn\<^sup>k *\<^sub>a conflict_assn\<^sup>d \<rightarrow>\<^sub>a conflict_assn\<close>
   (is \<open>_ \<in> _ *\<^sub>a ?c\<^sup>d \<rightarrow>\<^sub>a ?o\<close>)
 proof -
   have H: \<open>(uncurry remove1_wl_code, uncurry (RETURN \<circ>\<circ> remove1_mset))
-  \<in> nat_lit_assn\<^sup>k *\<^sub>a
-     (hr_comp (hr_comp (arl_assn nat_assn) (\<langle>nat_rel\<rangle>list_rel))
-       (list_mset_rel O
-        \<langle>nat_lit_rel\<rangle>mset_rel))\<^sup>d \<rightarrow>\<^sub>a hr_comp
-       (hr_comp (arl_assn nat_assn) {(l, l'). mset l = mset l'})
-       (list_mset_rel O \<langle>nat_lit_rel\<rangle>mset_rel)\<close>
+    \<in> (pure (uint32_nat_rel O nat_lit_rel))\<^sup>k *\<^sub>a
+   (hr_comp (hr_comp (arl_assn uint32_nat_assn) (\<langle>nat_rel\<rangle>list_rel))
+     (list_mset_rel O
+      \<langle>nat_lit_rel\<rangle>mset_rel))\<^sup>d \<rightarrow>\<^sub>a hr_comp
+    (hr_comp (arl_assn uint32_nat_assn) {(l, l'). mset l = mset l'})
+     (list_mset_rel O \<langle>nat_lit_rel\<rangle>mset_rel)\<close>
   (is \<open>_ \<in> _ *\<^sub>a ?c'\<^sup>d \<rightarrow>\<^sub>a ?o'\<close>)
     using remove1_wl_code.refine[FCOMP remove1_wl_remove1, FCOMP remove1_remove1_mset] .
-  have 1:
-    \<open>(\<exists>\<^sub>Aba bb. f bb * \<up> (bb = ba) * P ba) = (\<exists>\<^sub>Aba. f ba * P ba)\<close> for P :: \<open>'a \<Rightarrow> assn\<close> and f
-    by (sep_auto simp: ex_assn_def)
-  have [simp]:
-    \<open>(\<exists>\<^sub>Aba bb. f bb * \<up> (bb = ba \<and> P ba)) = (\<exists>\<^sub>Aba. f ba * \<up> (P ba))\<close> for P :: \<open>'a \<Rightarrow> bool\<close> and f
-    unfolding import_param_3 mult.assoc[symmetric] 1 ..
-  have 2: \<open>(\<exists>\<^sub>Aba bb.
-           is_array_list bb (aa, b) *
-           \<up> (list_all2 lit_of_natP bb ba \<and> a = mset ba))
-    = (\<exists>\<^sub>A bb.
-           is_array_list bb (aa, b) *
-           \<up> (\<exists>ba. list_all2 lit_of_natP bb ba \<and> a = mset ba))\<close>
-    for a aa b
-    apply (subst ex_assn_swap)
-    unfolding ex_assn_move_out[symmetric] ent_ex_up_swap ..
-  have 3: \<open>(\<exists>xs. mset xs = mset ba \<and>
-                   (\<exists>ys. mset ys = a \<and>
-                         list_all2 lit_of_natP xs ys)) \<longleftrightarrow>
-     (\<exists>b. list_all2 lit_of_natP ba b \<and> a = mset b)\<close> for a ba
-    using list_all2_reorder_left_invariance by fastforce
-  have "4a": \<open>(\<exists>\<^sub>Aba bb.
-           is_array_list bb (aa, b) *
-           \<up> (mset bb = mset ba \<and>
-              (\<exists>b. list_all2 lit_of_natP ba b \<and> a = mset b))) =
-      (\<exists>\<^sub>Abb.
-           is_array_list bb (aa, b) *
-           \<up> (\<exists>ba. (mset bb = mset ba \<and>
-              (\<exists>b. list_all2 lit_of_natP ba b \<and> a = mset b))))\<close> for a aa b
-    apply (subst ex_assn_swap)
-    apply (subst ex_assn_move_out[symmetric])+
-    apply (subst ent_ex_up_swap)
-    ..
-  have "4b": \<open>(\<exists>\<^sub>Aba bb.
-           is_array_list bb (aa, b) *
-           \<up> (list_all2 lit_of_natP bb ba \<and> a = mset ba)) =
-     (\<exists>\<^sub>Abb.
-           is_array_list bb (aa, b) *
-           \<up> (\<exists>ba. list_all2 lit_of_natP bb ba \<and> a = mset ba)) \<close>  for a aa b
-    apply (subst ex_assn_swap)
-    apply (subst ex_assn_move_out[symmetric])+
-    apply (subst ent_ex_up_swap)
-    ..
-  have 4: \<open>(\<exists>b. mset ba = mset b \<and>
-                  (\<exists>ba. list_all2 lit_of_natP b ba \<and>
-                        a = mset ba)) =
-           (\<exists>b. list_all2 lit_of_natP ba b \<and> a = mset b)\<close> for ba a
-    using list_all2_reorder_left_invariance by fastforce
+  have a_eq_ex_iff: \<open>(a = {#literal_of_nat (nat_of_uint32 x). x \<in># mset ba#})\<longleftrightarrow>
+         (\<exists>xs. mset xs = nat_of_uint32 `# mset ba \<and> a = literal_of_nat `# mset xs)\<close>
+       for a ba
+    using ex_mset[of \<open>nat_of_uint32 `# mset ba\<close>]
+    by (auto simp del: literal_of_nat.simps)
   have c: \<open>?c' = ?c\<close>
-    by (fastforce simp: hr_comp_def[abs_def] list_mset_rel_def mset_rel_def arl_assn_def
+    by (auto simp: hr_comp_def[abs_def] list_mset_rel_def mset_rel_def arl_assn_def
         p2rel_def rel2p_def[abs_def] br_def Collect_eq_comp rel_mset_def list_rel_def
-        list.rel_eq 2 3)
+        list.rel_eq  uint32_nat_rel_def nat_lit_rel_def
+        list_all2_op_eq_map_right_iff' unat_lit_rel_def lit_of_natP_def
+          ex_assn_def_pure_eq_middle2
+         ex_assn_def_pure_eq_middle3
+         eq_commute a_eq_ex_iff
+        simp del: literal_of_nat.simps
+        intro!: ext)
+   have ex_iff: \<open>(\<exists>xs. mset xs = nat_of_uint32 `# mset ba \<and> a = literal_of_nat `# mset xs) \<longleftrightarrow>
+         (\<exists>b. mset b = nat_of_uint32 `# mset ba \<and> (\<exists>xs. mset b = mset xs \<and> a = literal_of_nat `# mset xs))\<close>
+    for a ba bb
+    using ex_mset[of \<open>nat_of_uint32 `# mset ba\<close>]
+    by (auto simp del: literal_of_nat.simps)
+
   have o': \<open>?o' = ?o\<close>
-    by (fastforce simp: hr_comp_def[abs_def] list_mset_rel_def mset_rel_def arl_assn_def
-        list_rel_def list.rel_eq 3 "4a" "4b" 4 p2rel_def rel2p_def[abs_def] br_def Collect_eq_comp
-        rel_mset_def)
+    by (auto simp: hr_comp_def[abs_def] list_mset_rel_def mset_rel_def arl_assn_def
+        p2rel_def rel2p_def[abs_def] br_def Collect_eq_comp rel_mset_def list_rel_def
+        list.rel_eq  uint32_nat_rel_def nat_lit_rel_def
+        list_all2_op_eq_map_right_iff' unat_lit_rel_def lit_of_natP_def
+          ex_assn_def_pure_eq_middle2
+         ex_assn_def_pure_eq_middle3
+         eq_commute a_eq_ex_iff ex_assn_skip_first2 ex_iff
+        simp del: literal_of_nat.simps
+        intro!: ext)
 
   show ?thesis
-    using H unfolding c o' op_mset_delete_def .
+    using H unfolding c o' op_mset_delete_def unat_lit_rel_def .
 qed
 
 definition maximum_level :: \<open>(nat, nat) ann_lits \<Rightarrow> nat literal list \<Rightarrow> nat\<close> where
@@ -841,7 +944,7 @@ definition maximum_level :: \<open>(nat, nat) ann_lits \<Rightarrow> nat literal
 
 sepref_definition maximum_level_code
   is \<open>uncurry (RETURN oo (maximum_level :: (nat, nat) ann_lits \<Rightarrow> nat literal list \<Rightarrow> nat))\<close>
-  :: \<open>pair_nat_ann_lits_assn\<^sup>k *\<^sub>a (arl_assn nat_lit_assn)\<^sup>k \<rightarrow>\<^sub>a nat_assn\<close>
+  :: \<open>pair_nat_ann_lits_assn\<^sup>k *\<^sub>a (arl_assn unat_lit_assn)\<^sup>k \<rightarrow>\<^sub>a nat_assn\<close>
   unfolding maximum_level_def
   by sepref
 
@@ -927,20 +1030,32 @@ qed
 
 lemma is_in_arl_code_op_list_contains[sepref_fr_rules]:
   \<open>(uncurry is_in_arl_code, uncurry (RETURN oo op_list_contains)) \<in>
-    nat_lit_assn\<^sup>k *\<^sub>a (arl_assn nat_lit_assn)\<^sup>k \<rightarrow>\<^sub>a bool_assn\<close>
+    unat_lit_assn\<^sup>k *\<^sub>a (arl_assn unat_lit_assn)\<^sup>k \<rightarrow>\<^sub>a bool_assn\<close>
 proof -
   have 1: \<open>(uncurry is_in_arl, uncurry (RETURN oo op_list_contains)) \<in>
    Id \<times>\<^sub>r (\<langle>Id\<rangle>list_rel) \<rightarrow>\<^sub>f \<langle>bool_rel\<rangle> nres_rel\<close>
     by (rule is_in_arl_op_list_contains) (auto simp: IS_LEFT_UNIQUE_def)
-  have 2: \<open>hr_comp (arl_assn nat_lit_assn) (\<langle>Id\<rangle>list_rel) = arl_assn nat_lit_assn\<close>
+  have 2: \<open>hr_comp (arl_assn unat_lit_assn) (\<langle>Id\<rangle>list_rel) = arl_assn unat_lit_assn\<close>
     by (auto)
   show ?thesis
     using is_in_arl_code.refine[FCOMP 1] unfolding 2 .
 qed
 
+lemma [safe_constraint_rules]: \<open>is_pure (unat_lit_assn)\<close>
+  by auto
+
+text \<open>TODO Move\<close>
+instantiation uint32 :: default
+begin
+definition default_uint32 :: uint32 where
+  \<open>default_uint32 = 0\<close>
+instance
+  ..
+end
+
 sepref_definition union_mset_list_fold_code
   is \<open>uncurry (RETURN oo union_mset_list_fold)\<close>
-  :: \<open>(arl_assn nat_lit_assn)\<^sup>d *\<^sub>a (arl_assn nat_lit_assn)\<^sup>k \<rightarrow>\<^sub>a arl_assn nat_lit_assn\<close>
+  :: \<open>(arl_assn unat_lit_assn)\<^sup>d *\<^sub>a (arl_assn unat_lit_assn)\<^sup>k \<rightarrow>\<^sub>a arl_assn unat_lit_assn\<close>
   unfolding union_mset_list_fold_def
   by sepref
 
@@ -1204,7 +1319,7 @@ lemma watched_by_nth_watched_app':
 sepref_definition (in -) find_decomp_wl_imp_code
   is \<open>uncurry2 (find_decomp_wl_imp)\<close>
   :: \<open>[\<lambda>((M, D), L). M \<noteq> []]\<^sub>a
-         pair_nat_ann_lits_assn\<^sup>d *\<^sub>a conflict_assn\<^sup>k *\<^sub>a nat_lit_assn\<^sup>k
+         pair_nat_ann_lits_assn\<^sup>d *\<^sub>a conflict_assn\<^sup>k *\<^sub>a unat_lit_assn\<^sup>k
     \<rightarrow> pair_nat_ann_lits_assn\<close>
   unfolding find_decomp_wl_imp_def get_maximum_level_remove_def[symmetric] PR_CONST_def
   supply [[goals_limit=1]]
@@ -1231,24 +1346,31 @@ lemma nth_ll_watched_app:
   unfolding watched_app_def nth_ll_def
   by (fastforce simp: fref_def map_fun_rel_def prod_rel_def nres_rel_def p2rel_def lit_of_natP_def)
 
+ 
+lemma nth_aa_hnr_u[sepref_fr_rules]:
+  assumes p: \<open>is_pure R\<close>
+  shows
+    \<open>(uncurry2 (\<lambda>xs i. nth_aa xs (nat_of_uint32 i)), uncurry2 (RETURN \<circ>\<circ>\<circ> nth_ll)) \<in>
+       [\<lambda>((l,i),j). i < length l \<and> j < length_ll l i]\<^sub>a
+       (arrayO_assn (arl_assn R))\<^sup>k *\<^sub>a uint32_nat_assn\<^sup>k *\<^sub>a nat_assn\<^sup>k \<rightarrow> R\<close>
+  supply nth_aa_hnr[to_hnr, sep_heap_rules]
+  using assms
+  by sepref_to_hoare (sep_auto simp: uint32_nat_rel_def br_def)
+ 
 lemma nth_aa_watched_app[sepref_fr_rules]:
-  \<open>(uncurry2 nth_aa, uncurry2 (RETURN ooo op_watched_app)) \<in>
+  \<open>(uncurry2 (\<lambda>xs i. nth_aa xs (nat_of_uint32 i)), uncurry2 (RETURN ooo op_watched_app)) \<in>
    [\<lambda>((W, L), i). L \<in> snd ` D\<^sub>0 \<and> i < length (W L)]\<^sub>a
-     array_watched_assn\<^sup>k *\<^sub>a nat_lit_assn\<^sup>k *\<^sub>a nat_assn\<^sup>k \<rightarrow> nat_assn\<close>
+     array_watched_assn\<^sup>k *\<^sub>a unat_lit_assn\<^sup>k *\<^sub>a nat_assn\<^sup>k \<rightarrow> nat_assn\<close>
   (is \<open>?c \<in> [?pre]\<^sub>a ?im \<rightarrow> ?f\<close>)
 proof -
   have P: \<open>is_pure nat_assn\<close>
     by auto
-  have H: \<open>(uncurry2 nth_aa, uncurry2 (RETURN \<circ>\<circ>\<circ> op_watched_app))
-  \<in> [comp_PRE ((\<langle>Id\<rangle>map_fun_rel D\<^sub>0 \<times>\<^sub>r nat_lit_rel) \<times>\<^sub>r nat_rel)
-       (\<lambda>((W, L), i). L \<in> snd ` D\<^sub>0)
-       (\<lambda>_ ((l, i), j). i < length l \<and> j < length_ll l i)
-       (\<lambda>_. True)]\<^sub>a hrp_comp
-                       ((arrayO_assn (arl_assn nat_assn))\<^sup>k *\<^sub>a nat_assn\<^sup>k *\<^sub>a nat_assn\<^sup>k)
-                       ((\<langle>Id\<rangle>map_fun_rel D\<^sub>0 \<times>\<^sub>r nat_lit_rel) \<times>\<^sub>r nat_rel) \<rightarrow>
-                    hr_comp nat_assn nat_rel\<close>
+  have H: \<open>(uncurry2 (\<lambda>xs i. nth_aa xs (nat_of_uint32 i)), uncurry2 (RETURN \<circ>\<circ>\<circ> watched_app))
+  \<in> [comp_PRE (\<langle>Id\<rangle>map_fun_rel D\<^sub>0 \<times>\<^sub>f p2rel lit_of_natP \<times>\<^sub>f nat_rel) (\<lambda>((W, L), i). L \<in> snd ` D\<^sub>0) (\<lambda>_ ((l, i), j). i < length l \<and> j < length_ll l i)
+       (\<lambda>_. True)]\<^sub>a hrp_comp ((arrayO_assn (arl_assn nat_assn))\<^sup>k *\<^sub>a uint32_nat_assn\<^sup>k *\<^sub>a nat_assn\<^sup>k)
+                       (\<langle>Id\<rangle>map_fun_rel D\<^sub>0 \<times>\<^sub>f p2rel lit_of_natP \<times>\<^sub>f nat_rel) \<rightarrow> hr_comp nat_assn nat_rel\<close>
     (is \<open>_ \<in> [?pre']\<^sub>a ?im' \<rightarrow> ?f'\<close>)
-    using hfref_compI_PRE_aux[OF nth_aa_hnr nth_ll_watched_app, OF P]
+    using hfref_compI_PRE_aux[OF nth_aa_hnr_u nth_ll_watched_app, OF P]
     unfolding op_watched_app_def .
 
   have 1: \<open>?pre' = ?pre\<close>
@@ -1258,39 +1380,46 @@ proof -
         simp del: literal_of_nat.simps)
 
   have 2: \<open>?im' = ?im\<close>
-    unfolding prod_hrp_comp by (auto simp: hrp_comp_def hr_comp_def)
+    unfolding prod_hrp_comp by (auto simp: hrp_comp_def hr_comp_def nat_lit_rel_def p2rel_def
+        unat_lit_rel_def hr_comp_pure)
   have 3: \<open>?f' = ?f\<close>
     by (auto simp: hrp_comp_def hr_comp_def)
 
   show ?thesis
-    using H unfolding 1 2 3  .
+    using H unfolding 1 2 3 op_watched_app_def .
 qed
 
+lemma length_aa_hnr_u[sepref_fr_rules]: 
+  \<open>(uncurry (\<lambda>xs i. length_aa xs (nat_of_uint32 i)), uncurry (RETURN \<circ>\<circ> length_ll)) \<in>
+     [\<lambda>(xs, i). i < length xs]\<^sub>a (arrayO_assn (arl_assn R))\<^sup>k *\<^sub>a uint32_nat_assn\<^sup>k \<rightarrow> nat_assn\<close>
+  by sepref_to_hoare (sep_auto simp: uint32_nat_rel_def br_def)
+    
 lemma length_aa_length_ll_f[sepref_fr_rules]:
-  \<open>(uncurry length_aa, uncurry (RETURN oo length_ll_f)) \<in>
+  \<open>(uncurry (\<lambda>xs i. length_aa xs (nat_of_uint32 i)), uncurry (RETURN oo length_ll_f)) \<in>
    [\<lambda>(W, L). L \<in> snd ` D\<^sub>0]\<^sub>a
-     array_watched_assn\<^sup>k *\<^sub>a nat_lit_assn\<^sup>k \<rightarrow> nat_assn\<close>
+     array_watched_assn\<^sup>k *\<^sub>a unat_lit_assn\<^sup>k \<rightarrow> nat_assn\<close>
   (is \<open>?c \<in> [?pre]\<^sub>a ?im \<rightarrow> ?f\<close>)
 proof -
   have P: \<open>is_pure nat_assn\<close>
     by auto
-  have H: \<open>(uncurry length_aa, uncurry (RETURN \<circ>\<circ> length_ll_f))
+  have H: \<open>(uncurry (\<lambda>xs i. length_aa xs (nat_of_uint32 i)), uncurry (RETURN \<circ>\<circ> length_ll_f))
        \<in> [comp_PRE
             (\<langle>Id\<rangle>map_fun_rel D\<^sub>0 \<times>\<^sub>r nat_lit_rel)
             (\<lambda>(W, L). L \<in> snd ` D\<^sub>0)
             (\<lambda>_ (xs, i). i < length xs)
             (\<lambda>_. True)]\<^sub>a hrp_comp
-                            ((arrayO_assn (arl_assn nat_assn))\<^sup>k *\<^sub>a nat_assn\<^sup>k)
+                            ((arrayO_assn (arl_assn nat_assn))\<^sup>k *\<^sub>a uint32_nat_assn\<^sup>k)
                             (\<langle>Id\<rangle>map_fun_rel D\<^sub>0 \<times>\<^sub>r nat_lit_rel) \<rightarrow>
           hr_comp nat_assn nat_rel\<close>
     (is \<open>_ \<in> [?pre']\<^sub>a ?im' \<rightarrow> ?f'\<close>)
-    using hfref_compI_PRE_aux[OF length_aa_hnr length_ll_length_ll_f]
+    using hfref_compI_PRE_aux[OF length_aa_hnr_u length_ll_length_ll_f]
     unfolding op_watched_app_def .
 
   have 1: \<open>?pre' = ?pre\<close>
     using ex_list_watched
     by (fastforce simp: comp_PRE_def prod_rel_def_internal relAPP_def map_fun_rel_def[abs_def]
         p2rel_def lit_of_natP_def literal_of_neq_eq_nat_of_lit_eq_iff length_ll_def
+        nat_lit_rel_def
         simp del: literal_of_nat.simps)
 
   have 2: \<open>?im' = ?im\<close>
@@ -1299,7 +1428,7 @@ proof -
     by (auto simp: hrp_comp_def hr_comp_def)
 
   show ?thesis
-    using H unfolding 1 2 3  .
+    using H unfolding 1 2 3 .
 qed
 
 
@@ -1315,28 +1444,37 @@ lemma delete_index_and_swap_ll_delete_index_and_swap_update:
       \<langle>\<langle>Id\<rangle>map_fun_rel D\<^sub>0\<rangle>nres_rel\<close>
   by (auto simp: delete_index_and_swap_ll_def uncurry_def fref_def nres_rel_def
       delete_index_and_swap_update_def map_fun_rel_def p2rel_def lit_of_natP_def
-      nth_list_update'
+      nth_list_update' nat_lit_rel_def
       simp del: literal_of_nat.simps)
 
+thm delete_index_and_swap_aa_ll_hnr[to_hnr, unfolded hn_refine_def, simplified]
+lemma (in-) delete_index_and_swap_aa_ll_hnr_u:
+  assumes \<open>is_pure R\<close>
+  shows \<open>(uncurry2 (\<lambda>xs i. delete_index_and_swap_aa xs (nat_of_uint32 i)), uncurry2 (RETURN ooo delete_index_and_swap_ll))
+     \<in> [\<lambda>((l,i), j). i < length l \<and> j < length_ll l i]\<^sub>a (arrayO_assn (arl_assn R))\<^sup>d *\<^sub>a uint32_nat_assn\<^sup>k *\<^sub>a nat_assn\<^sup>k
+         \<rightarrow> (arrayO_assn (arl_assn R))\<close>
+  using assms unfolding delete_index_and_swap_aa_def
+  by sepref_to_hoare (sep_auto dest: le_length_ll_nemptyD
+      simp: delete_index_and_swap_ll_def update_ll_def last_ll_def set_butlast_ll_def
+      length_ll_def[symmetric] uint32_nat_rel_def br_def)
+
 lemma delete_index_and_swap_aa_hnr[sepref_fr_rules]:
-  shows \<open>(uncurry2 delete_index_and_swap_aa, uncurry2 (RETURN ooo delete_index_and_swap_update))
+  shows \<open>(uncurry2 (\<lambda>xs i j. delete_index_and_swap_aa xs (nat_of_uint32 i) j), uncurry2 (RETURN ooo delete_index_and_swap_update))
      \<in> [\<lambda>((W,L), j). L \<in> snd ` D\<^sub>0 \<and> j < length (W L)]\<^sub>a
-        array_watched_assn\<^sup>d *\<^sub>a nat_lit_assn\<^sup>k *\<^sub>a nat_assn\<^sup>k \<rightarrow> array_watched_assn\<close>
+        array_watched_assn\<^sup>d *\<^sub>a unat_lit_assn\<^sup>k *\<^sub>a nat_assn\<^sup>k \<rightarrow> array_watched_assn\<close>
     (is \<open>?a \<in> [?pre]\<^sub>a ?init \<rightarrow> ?post\<close>)
 proof -
-  have H: \<open>(uncurry2 delete_index_and_swap_aa, uncurry2 (RETURN \<circ>\<circ>\<circ> delete_index_and_swap_update))
-  \<in> [comp_PRE ((\<langle>Id\<rangle>map_fun_rel D\<^sub>0 \<times>\<^sub>r nat_lit_rel) \<times>\<^sub>r nat_rel) (\<lambda>((W, L), i). L \<in> snd ` D\<^sub>0)
-       (\<lambda>x y. case y of (x, xa) \<Rightarrow> (case x of (l, i) \<Rightarrow> \<lambda>j. i < length l \<and> j < length_ll l i) xa)
+  have H: \<open>(uncurry2 (\<lambda>xs i. delete_index_and_swap_aa xs (nat_of_uint32 i)), uncurry2 (RETURN \<circ>\<circ>\<circ> delete_index_and_swap_update))
+  \<in> [comp_PRE (\<langle>Id\<rangle>map_fun_rel D\<^sub>0 \<times>\<^sub>f nat_lit_rel \<times>\<^sub>f nat_rel) (\<lambda>((W, L), i). L \<in> snd ` D\<^sub>0) (\<lambda>x y. case y of (x, xa) \<Rightarrow> (case x of (l, i) \<Rightarrow> \<lambda>j. i < length l \<and> j < length_ll l i) xa)
        (\<lambda>x. nofail (uncurry2 (RETURN \<circ>\<circ>\<circ> delete_index_and_swap_update)
-                      x))]\<^sub>a hrp_comp ((arrayO_assn (arl_assn nat_assn))\<^sup>d *\<^sub>a nat_assn\<^sup>k *\<^sub>a nat_assn\<^sup>k)
-                              ((\<langle>Id\<rangle>map_fun_rel D\<^sub>0 \<times>\<^sub>r nat_lit_rel) \<times>\<^sub>r
-                               nat_rel) \<rightarrow> hr_comp (arrayO_assn (arl_assn nat_assn)) (\<langle>Id\<rangle>map_fun_rel D\<^sub>0)
+                      x))]\<^sub>a hrp_comp ((arrayO_assn (arl_assn nat_assn))\<^sup>d *\<^sub>a uint32_nat_assn\<^sup>k *\<^sub>a nat_assn\<^sup>k)
+                              (\<langle>Id\<rangle>map_fun_rel D\<^sub>0 \<times>\<^sub>f nat_lit_rel \<times>\<^sub>f nat_rel) \<rightarrow> hr_comp (arrayO_assn (arl_assn nat_assn)) (\<langle>Id\<rangle>map_fun_rel D\<^sub>0)
 \<close>
     (is \<open>?a \<in> [?pre']\<^sub>a ?init' \<rightarrow> ?post'\<close>)
-    using hfref_compI_PRE[OF delete_index_and_swap_aa_ll_hnr
+    using hfref_compI_PRE[OF delete_index_and_swap_aa_ll_hnr_u
         delete_index_and_swap_ll_delete_index_and_swap_update, of nat_assn] by simp
   have b: \<open>\<exists>bb. (bb, b) \<in> nat_lit_rel\<close> for b
-    apply (auto simp: p2rel_def lit_of_natP_def Pos_div2_iff Neg_div2_iff )
+    apply (auto simp: p2rel_def lit_of_natP_def Pos_div2_iff Neg_div2_iff nat_lit_rel_def)
     using even_Suc by blast
   have ba_length_a_b: \<open>ba < length (a b)\<close>
     if bN: \<open>b \<in># N\<^sub>1\<close> and
@@ -1355,7 +1493,7 @@ proof -
     obtain bb where bb: \<open>(bb, b) \<in> nat_lit_rel\<close>
       using b[of b] by blast
     show ?thesis
-      using H[of aa bb] aa bb aa_b_a_b by (auto simp: p2rel_def lit_of_natP_def)
+      using H[of aa bb] aa bb aa_b_a_b by (auto simp: p2rel_def lit_of_natP_def nat_lit_rel_def)
   qed
 
   have pre: \<open>?pre' = ?pre\<close>
@@ -1363,11 +1501,11 @@ proof -
         image_image ba_length_a_b
         Pos_div2_iff Neg_div2_iff all_conj_distrib length_ll_def
         intro!: ext split: if_splits)
-    by (auto simp: p2rel_def lit_of_natP_def split: if_splits)
+    by (auto simp: p2rel_def nat_lit_rel_def lit_of_natP_def split: if_splits)
 
   have
     1: \<open>hrp_comp (nat_assn\<^sup>k) nat_rel = nat_assn\<^sup>k\<close> and
-    2: \<open>hrp_comp (nat_assn\<^sup>k) nat_lit_rel = nat_lit_assn\<^sup>k\<close>
+    2: \<open>hrp_comp (uint32_nat_assn\<^sup>k) nat_lit_rel = unat_lit_assn\<^sup>k\<close>
      by (auto simp: hrp_comp_def)
   have init: \<open>?init' = ?init\<close>
     unfolding prod_hrp_comp 1 2 hrp_comp_dest by blast
@@ -1375,54 +1513,81 @@ proof -
   have post: \<open>?post' = ?post\<close>
     by simp
   show ?thesis
-    using H unfolding pre init
-    .
+    using H unfolding pre init .
 qed
 
-definition append_update :: "('a \<Rightarrow> 'b list) \<Rightarrow> 'a \<Rightarrow> 'b \<Rightarrow> 'a \<Rightarrow> 'b list" where
-  \<open>append_update W L a = W(L:= W L @ [a])\<close>
+definition append_update :: "('a \<Rightarrow> 'b list) \<Rightarrow> 'a \<Rightarrow> 'b \<Rightarrow> 'a \<Rightarrow> 'b list"  where
+  \<open>append_update W L a = W(L:= W (L) @ [a])\<close>
 
 lemma append_ll_append_update:
-  \<open>(uncurry2 (RETURN ooo append_ll), uncurry2 (RETURN ooo append_update))
+  \<open>(uncurry2 (RETURN ooo (\<lambda>xs i j. append_ll xs (nat_of_uint32 i) j)), uncurry2 (RETURN ooo append_update))
   \<in>  [\<lambda>((W, L), i). L \<in> snd ` D\<^sub>0]\<^sub>f
-     (\<langle>Id\<rangle>map_fun_rel D\<^sub>0 \<times>\<^sub>r nat_lit_rel) \<times>\<^sub>r nat_rel \<rightarrow> \<langle>\<langle>Id\<rangle>map_fun_rel D\<^sub>0\<rangle>nres_rel\<close>
+     \<langle>Id\<rangle>map_fun_rel D\<^sub>0 \<times>\<^sub>f unat_lit_rel \<times>\<^sub>f nat_rel \<rightarrow> \<langle>\<langle>Id\<rangle>map_fun_rel D\<^sub>0\<rangle>nres_rel\<close>
   by (auto simp: append_ll_def uncurry_def fref_def nres_rel_def
       delete_index_and_swap_update_def map_fun_rel_def p2rel_def lit_of_natP_def
-      nth_list_update' append_update_def
+      nth_list_update' append_update_def nat_lit_rel_def unat_lit_rel_def br_def
+      uint32_nat_rel_def
       simp del: literal_of_nat.simps)
 
+
+lemma append_aa_hnr_u:
+  fixes R ::  \<open>'a \<Rightarrow> 'b :: {heap, default} \<Rightarrow> assn\<close>
+  assumes p: \<open>is_pure R\<close>
+  shows
+    \<open>(uncurry2 (\<lambda>xs i. append_el_aa xs (nat_of_uint32 i)), uncurry2 (RETURN \<circ>\<circ>\<circ> (\<lambda>xs i. append_ll xs (nat_of_uint32 i)))) \<in>
+     [\<lambda>((l,i),x). nat_of_uint32 i < length l]\<^sub>a (arrayO_assn (arl_assn R))\<^sup>d *\<^sub>a uint32_assn\<^sup>k *\<^sub>a R\<^sup>k \<rightarrow> (arrayO_assn (arl_assn R))\<close>
+proof -
+  obtain R' where R: \<open>the_pure R = R'\<close> and R': \<open>R = pure R'\<close>
+    using p by fastforce
+  have [simp]: \<open>(\<exists>\<^sub>Ax. arrayO_assn (arl_assn R) a ai * R x r * true * \<up> (x = a ! ba ! b)) =
+     (arrayO_assn (arl_assn R) a ai * R (a ! ba ! b) r * true)\<close> for a ai ba b r
+    by (auto simp: ex_assn_def)
+  show ?thesis -- \<open>TODO tune proof\<close>
+    apply sepref_to_hoare
+    apply (sep_auto simp: append_el_aa_def uint32_nat_rel_def br_def)
+     apply (simp add: arrayO_except_assn_def)
+     apply (rule sep_auto_is_stupid[OF p])
+    apply (sep_auto simp: array_assn_def is_array_def append_ll_def)
+    apply (simp add: arrayO_except_assn_array0[symmetric] arrayO_except_assn_def)
+    apply (subst_tac (2) i = \<open>nat_of_uint32 ba\<close> in heap_list_all_nth_remove1)
+     apply (solves \<open>simp\<close>)
+    apply (simp add: array_assn_def is_array_def)
+    apply (rule_tac x=\<open>p[nat_of_uint32 ba := (ab, bc)]\<close> in ent_ex_postI)
+    apply (subst_tac (2)xs'=a and ys'=p in heap_list_all_nth_cong)
+      apply (solves \<open>auto\<close>)[2]
+    apply (auto simp: star_aci)
+    done
+qed
+
 lemma append_el_aa_hnr[sepref_fr_rules]:
-  shows \<open>(uncurry2 append_el_aa, uncurry2 (RETURN ooo append_update))
+  shows \<open>(uncurry2 (\<lambda>xs i j. append_el_aa xs (nat_of_uint32 i) j), uncurry2 (RETURN ooo append_update))
      \<in> [\<lambda>((W,L), j). L \<in> snd ` D\<^sub>0]\<^sub>a
-        array_watched_assn\<^sup>d *\<^sub>a nat_lit_assn\<^sup>k *\<^sub>a nat_assn\<^sup>k \<rightarrow> array_watched_assn\<close>
+        array_watched_assn\<^sup>d *\<^sub>a unat_lit_assn\<^sup>k *\<^sub>a nat_assn\<^sup>k \<rightarrow> array_watched_assn\<close>
     (is \<open>?a \<in> [?pre]\<^sub>a ?init \<rightarrow> ?post\<close>)
 proof -
-  have H: \<open>(uncurry2 append_el_aa,
-   uncurry2 (RETURN \<circ>\<circ>\<circ> append_update))
-  \<in> [comp_PRE ((\<langle>Id\<rangle>map_fun_rel D\<^sub>0 \<times>\<^sub>r nat_lit_rel) \<times>\<^sub>r nat_rel)
-       (\<lambda>((W, L), i). L \<in> snd ` D\<^sub>0)
-       (\<lambda>x y. case y of (x, xa) \<Rightarrow> (case x of (l, i) \<Rightarrow> \<lambda>x. i < length l) xa)
-       (\<lambda>x. nofail (uncurry2 (RETURN \<circ>\<circ>\<circ> append_update) x))]\<^sub>a
-    hrp_comp ((arrayO_assn (arl_assn nat_assn))\<^sup>d *\<^sub>a nat_assn\<^sup>k *\<^sub>a nat_assn\<^sup>k)
-      ((\<langle>Id\<rangle>map_fun_rel D\<^sub>0 \<times>\<^sub>r nat_lit_rel) \<times>\<^sub>r nat_rel) \<rightarrow>
-    hr_comp (arrayO_assn (arl_assn nat_assn)) (\<langle>Id\<rangle>map_fun_rel D\<^sub>0)
-\<close>
+  have H: \<open> (uncurry2 (\<lambda>xs i. append_el_aa xs (nat_of_uint32 i)), uncurry2 (RETURN \<circ>\<circ>\<circ> append_update))
+  \<in> [comp_PRE (\<langle>Id\<rangle>map_fun_rel D\<^sub>0 \<times>\<^sub>f unat_lit_rel \<times>\<^sub>f nat_rel) (\<lambda>((W, L), i). L \<in> snd ` D\<^sub>0) (\<lambda>x y. case y of (x, xa) \<Rightarrow> (case x of (l, i) \<Rightarrow> \<lambda>x. nat_of_uint32 i < length l) xa)
+       (\<lambda>x. nofail (uncurry2 (RETURN \<circ>\<circ>\<circ> append_update)
+                      x))]\<^sub>a hrp_comp ((arrayO_assn (arl_assn nat_assn))\<^sup>d *\<^sub>a uint32_assn\<^sup>k *\<^sub>a nat_assn\<^sup>k)
+                              (\<langle>Id\<rangle>map_fun_rel D\<^sub>0 \<times>\<^sub>f unat_lit_rel \<times>\<^sub>f nat_rel) \<rightarrow> hr_comp (arrayO_assn (arl_assn nat_assn)) (\<langle>Id\<rangle>map_fun_rel D\<^sub>0)
+     \<close>
     (is \<open>?a \<in> [?pre']\<^sub>a ?init' \<rightarrow> ?post'\<close>)
-    using hfref_compI_PRE[OF append_aa_hnr
+    using hfref_compI_PRE[OF append_aa_hnr_u
         append_ll_append_update, of nat_assn] by simp
   have b: \<open>\<exists>bb. (bb, b) \<in> nat_lit_rel\<close> for b
-    apply (auto simp: p2rel_def lit_of_natP_def Pos_div2_iff Neg_div2_iff )
+    apply (auto simp: p2rel_def lit_of_natP_def Pos_div2_iff Neg_div2_iff nat_lit_rel_def)
     using even_Suc by blast
 
   have pre: \<open>?pre' = ?pre\<close>
     apply (auto simp: comp_PRE_def map_fun_rel_def lit_of_natP_def image_image
         Pos_div2_iff Neg_div2_iff all_conj_distrib length_ll_def
         intro!: ext split: if_splits)
-    by (auto simp: p2rel_def lit_of_natP_def split: if_splits)
+    by (auto simp: p2rel_def lit_of_natP_def unat_lit_rel_def br_def nat_lit_rel_def uint32_nat_rel_def
+        split: if_splits)
 
   have
     1: \<open>hrp_comp (nat_assn\<^sup>k) nat_rel = nat_assn\<^sup>k\<close> and
-    2: \<open>hrp_comp (nat_assn\<^sup>k) nat_lit_rel = nat_lit_assn\<^sup>k\<close>
+    2: \<open>hrp_comp (uint32_assn\<^sup>k) unat_lit_rel = unat_lit_assn\<^sup>k\<close>
      by (auto simp: hrp_comp_def)
   have init: \<open>?init' = ?init\<close>
     unfolding prod_hrp_comp 1 2 hrp_comp_dest by blast
@@ -1430,8 +1595,7 @@ proof -
   have post: \<open>?post' = ?post\<close>
     by simp
   show ?thesis
-    using H unfolding pre init
-    .
+    using H unfolding pre init by blast
 qed
 
 lemma literals_to_update_wl_literals_to_update_wl_empty:
@@ -1522,12 +1686,13 @@ lemma Propagated_eq_ann_lit_of_pair_iff:
 
 lemma lit_and_ann_of_propagated_hnr[sepref_fr_rules]:
   \<open>(return o (\<lambda>L::ann_lit_wl. (fst L, the (snd L))), RETURN o lit_and_ann_of_propagated) \<in>
-   [\<lambda>L. \<not>is_decided L]\<^sub>a pair_nat_ann_lit_assn\<^sup>k \<rightarrow> (nat_lit_assn *assn nat_assn)\<close>
+   [\<lambda>L. \<not>is_decided L]\<^sub>a pair_nat_ann_lit_assn\<^sup>k \<rightarrow> (unat_lit_assn *assn nat_assn)\<close>
   apply sepref_to_hoare
   apply (rename_tac x x')
   apply (case_tac x)
   by (sep_auto simp: nat_ann_lit_rel_def p2rel_def lit_of_natP_def
-      Propagated_eq_ann_lit_of_pair_iff
+      Propagated_eq_ann_lit_of_pair_iff unat_lit_rel_def uint32_nat_rel_def Collect_eq_comp
+      br_def Collect_eq_comp nat_lit_rel_def
       simp del: literal_of_nat.simps)+
 
 definition op_mset_arl_empty :: "'a multiset" where
@@ -1541,7 +1706,7 @@ lemma arl_empty_op_mset_arl_empy[sepref_fr_rules]:
 
 text \<open>TODO move upper\<close>
 lemma (in -) id_list_of_mset[sepref_fr_rules]:
-  \<open>(return o id, list_of_mset) \<in> conflict_assn\<^sup>d \<rightarrow>\<^sub>a arl_assn nat_lit_assn\<close>
+  \<open>(return o id, list_of_mset) \<in> conflict_assn\<^sup>d \<rightarrow>\<^sub>a arl_assn unat_lit_assn\<close>
   by sepref_to_hoare (sep_auto simp: hr_comp_def list_of_mset_def arl_assn_def list_mset_rel_def
       br_def)
 
@@ -1558,7 +1723,7 @@ definition (in -) find_lit_of_max_level_wl_imp where
 term maximum_level_remove_code
 sepref_definition (in -) maximum_level_remove_code_array
   is \<open>uncurry2 (RETURN ooo maximum_level_remove)\<close>
-  :: \<open>pair_nat_ann_lits_assn\<^sup>k *\<^sub>a (array_assn nat_lit_assn)\<^sup>k *\<^sub>a nat_lit_assn\<^sup>k \<rightarrow>\<^sub>a nat_assn\<close>
+  :: \<open>pair_nat_ann_lits_assn\<^sup>k *\<^sub>a (array_assn unat_lit_assn)\<^sup>k *\<^sub>a unat_lit_assn\<^sup>k \<rightarrow>\<^sub>a nat_assn\<close>
   unfolding maximum_level_remove_def[abs_def]
   by sepref
 
@@ -1588,10 +1753,10 @@ definition (in -) remove1_and_add_first :: "nat literal \<Rightarrow> nat litera
 
 lemma (in -)find_first_eq_code_index[sepref_fr_rules]:
   \<open>(uncurry (\<lambda>xs a. find_first_eq_code a xs), uncurry (RETURN oo op_list_index)) \<in>
-      (arl_assn nat_lit_assn)\<^sup>k *\<^sub>a nat_lit_assn\<^sup>k \<rightarrow>\<^sub>a nat_assn\<close>
+      (arl_assn unat_lit_assn)\<^sup>k *\<^sub>a unat_lit_assn\<^sup>k \<rightarrow>\<^sub>a nat_assn\<close>
 proof -
   have 0: \<open>(uncurry (\<lambda>xs a. find_first_eq_code a xs), uncurry (\<lambda>xs a. find_first_eq a xs))
-  \<in> (arl_assn nat_assn)\<^sup>k *\<^sub>a nat_assn\<^sup>k \<rightarrow>\<^sub>a nat_assn\<close>
+  \<in> (arl_assn uint32_nat_assn)\<^sup>k *\<^sub>a uint32_nat_assn\<^sup>k \<rightarrow>\<^sub>a nat_assn\<close>
     using find_first_eq_code.refine by (sep_auto simp: hfref_def ac_simps)
   have 1: \<open>(uncurry (\<lambda>xs a. find_first_eq a xs), uncurry (RETURN oo index)) \<in>
         \<langle>nat_rel\<rangle>list_rel \<times>\<^sub>r nat_rel \<rightarrow>\<^sub>f \<langle>nat_rel\<rangle>nres_rel\<close>
@@ -1599,27 +1764,31 @@ proof -
   have \<open>list_all2 (\<lambda>x x'. (x, x') \<in> nat_lit_rel) a aa \<Longrightarrow>
        (b, ba) \<in> nat_lit_rel \<Longrightarrow> find_index (\<lambda>x. x = b) a = find_index (\<lambda>x. x = ba) aa\<close> for a aa b ba
     by (induction a aa rule: list_all2_induct)
-      (auto dest: lit_of_natP_same_rightD lit_of_natP_same_leftD p2relD)
+      (auto dest: lit_of_natP_same_rightD lit_of_natP_same_leftD p2relD simp: nat_lit_rel_def)
   then have 2: \<open>(uncurry (RETURN oo index), uncurry (RETURN oo index)) \<in>
         \<langle>nat_lit_rel\<rangle> list_rel \<times>\<^sub>r nat_lit_rel \<rightarrow>\<^sub>f \<langle>nat_rel\<rangle>nres_rel\<close>
     by (intro frefI nres_relI) (auto simp: index_def list_rel_def)
-  have 3: \<open>(hr_comp (hr_comp (arl_assn nat_assn) (\<langle>nat_rel\<rangle>list_rel)) (\<langle>nat_lit_rel\<rangle>list_rel)) =
-   arl_assn nat_lit_assn\<close>
-    by (auto simp: arl_assn_def)
+  have 3: \<open>(hr_comp (hr_comp (arl_assn uint32_nat_assn) (\<langle>nat_rel\<rangle>list_rel)) (\<langle>nat_lit_rel\<rangle>list_rel)) =
+   arl_assn unat_lit_assn\<close>
+    by (simp add: hr_comp_assoc list_rel_compp unat_lit_rel_def arl_assn_def)
+
+  have 4: \<open>uint32_nat_rel O nat_lit_rel = unat_lit_rel\<close>
+    by (auto simp: uint32_nat_rel_def br_def nat_lit_rel_def unat_lit_rel_def)
+
   show ?thesis
-    using 0[FCOMP 1, FCOMP 2] unfolding 3 by simp
+    using 0[FCOMP 1, FCOMP 2] unfolding 3 4 by simp
 qed
 
 sepref_definition (in -)remove1_and_add_first_code
   is \<open>uncurry2 (remove1_and_add_first)\<close>
-  :: \<open>nat_lit_assn\<^sup>k *\<^sub>a nat_lit_assn\<^sup>k *\<^sub>a (arl_assn nat_lit_assn)\<^sup>d \<rightarrow>\<^sub>a (arl_assn nat_lit_assn)\<close>
+  :: \<open>unat_lit_assn\<^sup>k *\<^sub>a unat_lit_assn\<^sup>k *\<^sub>a (arl_assn unat_lit_assn)\<^sup>d \<rightarrow>\<^sub>a (arl_assn unat_lit_assn)\<close>
   unfolding remove1_and_add_first_def
   by sepref
 
 lemma (in -)remove1_and_add_first_code_list_of_mset2[sepref_fr_rules]:
   \<open>(uncurry2 remove1_and_add_first_code, uncurry2 (list_of_mset2))
   \<in> [\<lambda>((L, L'), D). L \<in># D \<and> L' \<in># D \<and> L \<noteq> L' \<and> distinct_mset D]\<^sub>a
-     nat_lit_assn\<^sup>k *\<^sub>a nat_lit_assn\<^sup>k *\<^sub>a conflict_assn\<^sup>d \<rightarrow> arl_assn nat_lit_assn\<close>
+     unat_lit_assn\<^sup>k *\<^sub>a unat_lit_assn\<^sup>k *\<^sub>a conflict_assn\<^sup>d \<rightarrow> arl_assn unat_lit_assn\<close>
   (is \<open>_ \<in> [?P]\<^sub>a _ \<rightarrow> _\<close>)
 proof -
   have \<open>aa \<in> set ba \<Longrightarrow>
@@ -1658,13 +1827,13 @@ definition (in -) single_of_mset_imp :: \<open>'a list \<Rightarrow> 'a nres\<cl
 
 sepref_definition(in -) single_of_mset_imp_code
   is \<open>single_of_mset_imp\<close>
-  :: \<open>(arl_assn nat_lit_assn)\<^sup>d \<rightarrow>\<^sub>a nat_lit_assn\<close>
+  :: \<open>(arl_assn unat_lit_assn)\<^sup>d \<rightarrow>\<^sub>a unat_lit_assn\<close>
   unfolding single_of_mset_imp_def
   by sepref
 
 lemma (in -)single_of_mset_imp_code_single_of_mset[sepref_fr_rules]:
   \<open>(single_of_mset_imp_code, single_of_mset) \<in> [\<lambda>D. D \<noteq> {#} \<and> size D \<le> 1]\<^sub>a
-     conflict_assn\<^sup>d \<rightarrow> nat_lit_assn\<close>
+     conflict_assn\<^sup>d \<rightarrow> unat_lit_assn\<close>
 proof -
   have 1: \<open>(single_of_mset_imp, single_of_mset) \<in> [\<lambda>D. D \<noteq> {#} \<and> size D \<le> 1]\<^sub>f list_mset_rel \<rightarrow>
       \<langle>Id\<rangle> nres_rel\<close>
@@ -1695,9 +1864,10 @@ definition find_unassigned_lit_wl_D :: \<open>_\<close> where
 sepref_register N\<^sub>0'
 declare N_hnr'[sepref_fr_rules]
 
-lemma N_hnr[sepref_import_param]: "(N\<^sub>0,N\<^sub>0')\<in>\<langle>nat_lit_rel\<rangle>list_rel"
+lemma N_hnr[sepref_import_param]: "(N\<^sub>0,N\<^sub>0')\<in>\<langle>unat_lit_rel\<rangle>list_rel"
   unfolding N\<^sub>0'_def
-  by (induction N\<^sub>0) (auto simp del: literal_of_nat.simps simp: p2rel_def lit_of_natP_def)
+  by (induction N\<^sub>0) (auto simp del: literal_of_nat.simps simp: p2rel_def lit_of_natP_def
+      unat_lit_rel_def uint32_nat_rel_def nat_lit_rel_def br_def)
 
 lemma set_mset_lits_of_atms_of_mm_atms_of_ms_iff:
   \<open>set_mset (lits_of_atms_of_mm A) = set_mset N\<^sub>1 \<longleftrightarrow> atms_of_ms (set_mset A) = atms_of N\<^sub>1\<close>
