Weidenbach_Book/CDCL_Two_Watched_Literals_List_Watched_Domain.thy
@@ -1,5 +1,6 @@
 theory CDCL_Two_Watched_Literals_List_Watched_Domain
   imports CDCL_Two_Watched_Literals_List_Watched Array_Array_List Array_List_Array
+    WB_Word_Assn
 begin
 
 text \<open>We refine the implementation by adding a \<^emph>\<open>domain\<close> on the literals\<close>
@@ -12,10 +13,10 @@ subsubsection \<open>Functions and Types:\<close>
 
 type_synonym ann_lits_l = \<open>(nat, nat) ann_lits\<close>
 type_synonym clauses_to_update_ll = \<open>nat list\<close>
-type_synonym lit_queue_l = \<open>nat list\<close>
-type_synonym nat_trail = \<open>(nat \<times> nat option) list\<close>
-type_synonym clause_wl = \<open>nat array\<close>
-type_synonym unit_lits_wl = \<open>nat list list\<close>
+type_synonym lit_queue_l = \<open>uint32 list\<close>
+type_synonym nat_trail = \<open>(uint32 \<times> nat option) list\<close>
+type_synonym clause_wl = \<open>uint32 array\<close>
+type_synonym unit_lits_wl = \<open>uint32 list list\<close>
 
 type_synonym watched_wl = \<open>(nat array_list) array\<close>
 
@@ -79,11 +80,17 @@ lemma literal_of_nat_literal_of_nat_eq[iff]: \<open>literal_of_nat x = literal_o
 definition lit_of_natP where
   \<open>lit_of_natP L L' \<longleftrightarrow> literal_of_nat L = L'\<close>
 
-abbreviation nat_lit_rel :: "(nat \<times> nat literal) set" where
-  \<open>nat_lit_rel \<equiv> p2rel lit_of_natP\<close>
+definition nat_lit_rel :: "(nat \<times> nat literal) set" where
+  \<open>nat_lit_rel \<equiv> {(n, L). lit_of_natP n L}\<close>
 
 abbreviation nat_lit_assn :: "nat literal \<Rightarrow> nat \<Rightarrow> assn" where
   \<open>nat_lit_assn \<equiv> pure nat_lit_rel\<close>
+
+definition unat_lit_rel :: "(uint32 \<times> nat literal) set" where
+  \<open>unat_lit_rel \<equiv> uint32_nat_rel O nat_lit_rel\<close>
+
+abbreviation unat_lit_assn :: "nat literal \<Rightarrow> uint32 \<Rightarrow> assn" where
+  \<open>unat_lit_assn \<equiv> pure unat_lit_rel\<close>
 
 fun pair_of_ann_lit :: "('a, 'b) ann_lit \<Rightarrow> 'a literal \<times> 'b option" where
   \<open>pair_of_ann_lit (Propagated L D) = (L, Some D)\<close>
@@ -109,14 +116,39 @@ lemma nat_of_lit_eq_iff[iff]: \<open>nat_of_lit xa = nat_of_lit x \<longleftrigh
 lemma lit_of_natP_nat_of_lit_iff: \<open>lit_of_natP c a \<longleftrightarrow> c = nat_of_lit a\<close>
   by (cases a) (auto simp: lit_of_natP_def)
 
-type_synonym ann_lit_wl = \<open>nat \<times> nat option\<close>
+term \<open>\<lambda>R R'. {(a, b). \<exists>c d. (fst a, c) \<in> R \<and> (snd a, d) \<in> R' \<and>
+      b = ann_lit_of_pair (literal_of_nat c, d)}\<close>
+  
+definition ann_lit_rel:: "('a \<times> nat) set \<Rightarrow> ('b \<times> nat option) set \<Rightarrow>
+    (('a \<times> 'b) \<times> (nat, nat) ann_lit) set" where
+  ann_lit_rel_internal_def:
+  \<open>ann_lit_rel R R' = {(a, b). \<exists>c d. (fst a, c) \<in> R \<and> (snd a, d) \<in> R' \<and>
+      b = ann_lit_of_pair (literal_of_nat c, d)}\<close>
+
+type_synonym ann_lit_wl = \<open>uint32 \<times> nat option\<close>
 type_synonym ann_lits_wl = \<open>ann_lit_wl list\<close>
+term \<open> \<langle>uint32_nat_rel\<rangle>option_rel\<close>
 
 definition nat_ann_lit_rel :: "(ann_lit_wl \<times> (nat, nat) ann_lit) set" where
-  \<open>nat_ann_lit_rel = ({(a, b). b = ann_lit_of_pair ((\<lambda>(a,b). (literal_of_nat a, b)) a)})\<close>
+  nat_ann_lit_rel_internal_def: \<open>nat_ann_lit_rel = \<langle>uint32_nat_rel, \<langle>nat_rel\<rangle>option_rel\<rangle>ann_lit_rel\<close>
+
+lemma ann_lit_rel_def:
+  \<open>\<langle>R, R'\<rangle>ann_lit_rel = {(a, b). \<exists>c d. (fst a, c) \<in> R \<and> (snd a, d) \<in> R' \<and>
+      b = ann_lit_of_pair (literal_of_nat c, d)}\<close>
+  unfolding nat_ann_lit_rel_internal_def ann_lit_rel_internal_def relAPP_def ..
+
+lemma nat_ann_lit_rel_def:
+  \<open>nat_ann_lit_rel = {(a, b). b = ann_lit_of_pair ((\<lambda>(a,b). (literal_of_nat (nat_of_uint32 a), b)) a)}\<close>
+  unfolding nat_ann_lit_rel_internal_def ann_lit_rel_def
+  apply (auto simp: option_rel_def ex_disj_distrib uint32_nat_rel_def br_def)
+   apply (case_tac b)
+    apply auto
+   apply (case_tac b)
+   apply auto
+  done
 
 definition nat_ann_lits_rel :: "(ann_lits_wl \<times> (nat, nat) ann_lits) set" where
-  \<open>nat_ann_lits_rel = \<langle>(Id \<times>\<^sub>r \<langle>Id\<rangle>option_rel) O nat_ann_lit_rel\<rangle>list_rel\<close>
+  \<open>nat_ann_lits_rel = \<langle>nat_ann_lit_rel\<rangle>list_rel\<close>
 
 abbreviation pair_nat_ann_lit_assn :: "(nat, nat) ann_lit \<Rightarrow> ann_lit_wl \<Rightarrow> assn" where
   \<open>pair_nat_ann_lit_assn \<equiv> pure (nat_ann_lit_rel)\<close>
@@ -140,27 +172,38 @@ lemma lit_of_natP_same_leftD: \<open>lit_of_natP bi b \<Longrightarrow> lit_of_n
 
 subsection \<open>Refinement\<close>
 
+definition upperN :: nat where
+  \<open>upperN = 2 ^32\<close>
+
 text \<open>We start in a context where we have an initial set of literals. It should be
   a context, but this is not compatible with the refinement framework. It does only appear in
   the specifications.\<close>
 locale twl_array_code =
-  fixes N\<^sub>0 :: \<open>nat list\<close>
+  fixes N\<^sub>0 :: \<open>uint32 list\<close>
+  assumes \<open>\<forall>L \<in> set N\<^sub>0. nat_of_uint32 L < upperN\<close>
 begin
 
 text \<open>This is the \<^emph>\<open>completion\<close> of \<^term>\<open>N\<^sub>0\<close>, containing the positive and the negation of every
   literal of \<^term>\<open>N\<^sub>0\<close>:\<close>
-definition N\<^sub>0' where \<open>N\<^sub>0' = map literal_of_nat N\<^sub>0\<close>
+definition N\<^sub>0' where \<open>N\<^sub>0' = map (literal_of_nat o nat_of_uint32) N\<^sub>0\<close>
 definition N\<^sub>0'' where \<open>N\<^sub>0'' = mset N\<^sub>0'\<close>
 
 definition N\<^sub>1 where \<open>N\<^sub>1 = N\<^sub>0'' + uminus `# N\<^sub>0''\<close>
 
+lemma in_N1_less_than_upperN: \<open>L \<in># N\<^sub>1 \<Longrightarrow> nat_of_lit L < upperN\<close>
+  using twl_array_code_axioms unfolding twl_array_code_def
+  apply (auto simp: N\<^sub>1_def N\<^sub>0''_def N\<^sub>0'_def)
+    apply (metis Suc_lessI even_Suc even_numeral even_power upperN_def zero_less_numeral)
+  using less_imp_diff_less by blast
+
 sepref_register N\<^sub>1
-lemma list_assn_N\<^sub>0: \<open>list_assn (\<lambda>a c. \<up> ((c, a) \<in> nat_lit_rel)) N\<^sub>0' N\<^sub>0 = emp\<close>
+lemma list_assn_N\<^sub>0: \<open>list_assn (\<lambda>a c. \<up> ((c, a) \<in> unat_lit_rel)) N\<^sub>0' N\<^sub>0 = emp\<close>
   unfolding N\<^sub>0'_def
-  by (induction N\<^sub>0)  (auto simp del: literal_of_nat.simps simp: p2rel_def lit_of_natP_def)
+  by (induction N\<^sub>0) (auto simp del: literal_of_nat.simps simp: p2rel_def lit_of_natP_def
+   br_def Collect_eq_comp uint32_nat_rel_def unat_lit_rel_def nat_lit_rel_def)
 
 lemma N_hnr'[sepref_import_param]:
-  "(uncurry0 (return N\<^sub>0), uncurry0 (RETURN N\<^sub>0'))\<in>unit_assn\<^sup>k \<rightarrow>\<^sub>a list_assn nat_lit_assn"
+  "(uncurry0 (return N\<^sub>0), uncurry0 (RETURN N\<^sub>0'))\<in> unit_assn\<^sup>k \<rightarrow>\<^sub>a list_assn unat_lit_assn"
   by sepref_to_hoare (sep_auto simp: list_assn_N\<^sub>0)
 
 abbreviation D\<^sub>0 :: \<open>(nat \<times> nat literal) set\<close> where
@@ -171,10 +214,11 @@ definition length_ll_f where
 
 lemma length_ll_length_ll_f:
   \<open>(uncurry (RETURN oo length_ll), uncurry (RETURN oo length_ll_f)) \<in>
-     [\<lambda>(W, L). L \<in> snd ` D\<^sub>0]\<^sub>f ((\<langle>Id\<rangle>map_fun_rel D\<^sub>0) \<times>\<^sub>r p2rel lit_of_natP) \<rightarrow>
+     [\<lambda>(W, L). L \<in> snd ` D\<^sub>0]\<^sub>f ((\<langle>Id\<rangle>map_fun_rel D\<^sub>0) \<times>\<^sub>r nat_lit_rel) \<rightarrow>
        \<langle>nat_rel\<rangle> nres_rel\<close>
   unfolding length_ll_def length_ll_f_def
-  by (fastforce simp: fref_def map_fun_rel_def prod_rel_def nres_rel_def p2rel_def lit_of_natP_def)
+  by (fastforce simp: fref_def map_fun_rel_def prod_rel_def nres_rel_def p2rel_def lit_of_natP_def
+      nat_lit_rel_def)
 
 abbreviation array_watched_assn :: "(nat literal \<Rightarrow> nat list) \<Rightarrow> (nat array_list) array \<Rightarrow> assn" where
   \<open>array_watched_assn \<equiv> hr_comp (arrayO_assn (arl_assn nat_assn)) (\<langle>Id\<rangle>map_fun_rel D\<^sub>0)\<close>
@@ -230,39 +274,50 @@ proof -
     by blast
 qed
 
+definition length_aa_u :: \<open>('a::heap array_list) array \<Rightarrow> uint32 \<Rightarrow> nat Heap\<close> where
+  \<open>length_aa_u xs i = length_aa xs (nat_of_uint32 i)\<close>
+
+lemma length_aa_u_hnr[sepref_fr_rules]: \<open>(uncurry length_aa_u, uncurry (RETURN \<circ>\<circ> length_ll)) \<in>
+     [\<lambda>(xs, i). i < length xs]\<^sub>a (arrayO_assn (arl_assn R))\<^sup>k *\<^sub>a uint32_nat_assn\<^sup>k \<rightarrow> nat_assn\<close>
+  by sepref_to_hoare (sep_auto simp: uint32_nat_rel_def length_aa_u_def br_def)
+
+lemma hr_comp_uint32_nat_assn_nat_lit_rel[simp]:
+  \<open>hr_comp uint32_nat_assn nat_lit_rel = unat_lit_assn\<close>
+  by (auto simp: hrp_comp_def hr_comp_def uint32_nat_rel_def
+        lit_of_natP_def hr_comp_pure br_def unat_lit_rel_def)
+  
 lemma length_aa_length_ll_f[sepref_fr_rules]:
-  \<open>(uncurry length_aa, uncurry (RETURN oo length_ll_f)) \<in>
+  \<open>(uncurry length_aa_u, uncurry (RETURN oo length_ll_f)) \<in>
    [\<lambda>(W, L). L \<in> snd ` D\<^sub>0]\<^sub>a
-     array_watched_assn\<^sup>k *\<^sub>a nat_lit_assn\<^sup>k \<rightarrow> nat_assn\<close>
+     array_watched_assn\<^sup>k *\<^sub>a unat_lit_assn\<^sup>k \<rightarrow> nat_assn\<close>
   (is \<open>?c \<in> [?pre]\<^sub>a ?im \<rightarrow> ?f\<close>)
 proof -
   have P: \<open>is_pure nat_assn\<close>
     by auto
-  have H: \<open>(uncurry length_aa, uncurry (RETURN \<circ>\<circ> length_ll_f))
-       \<in> [comp_PRE
-            (\<langle>Id\<rangle>map_fun_rel D\<^sub>0 \<times>\<^sub>r nat_lit_rel)
-            (\<lambda>(W, L). L \<in> snd ` D\<^sub>0)
-            (\<lambda>_ (xs, i). i < length xs)
-            (\<lambda>_. True)]\<^sub>a hrp_comp
-                            ((arrayO_assn (arl_assn nat_assn))\<^sup>k *\<^sub>a nat_assn\<^sup>k)
-                            (\<langle>Id\<rangle>map_fun_rel D\<^sub>0 \<times>\<^sub>r nat_lit_rel) \<rightarrow>
-          hr_comp nat_assn nat_rel\<close>
+  have H: \<open>(uncurry length_aa_u, uncurry (RETURN \<circ>\<circ> length_ll_f))
+     \<in> [comp_PRE (\<langle>Id\<rangle>map_fun_rel D\<^sub>0 \<times>\<^sub>r nat_lit_rel)
+     (\<lambda>(W, L). L \<in> snd ` D\<^sub>0) (\<lambda>_ (xs, i). i < length xs)
+     (\<lambda>_. True)]\<^sub>a hrp_comp
+                     ((arrayO_assn (arl_assn nat_assn))\<^sup>k *\<^sub>a
+                      uint32_nat_assn\<^sup>k)
+                     (\<langle>Id\<rangle>map_fun_rel D\<^sub>0 \<times>\<^sub>r
+                      nat_lit_rel) \<rightarrow> hr_comp nat_assn nat_rel\<close>
     (is \<open>_ \<in> [?pre']\<^sub>a ?im' \<rightarrow> ?f'\<close>)
-    using hfref_compI_PRE_aux[OF length_aa_hnr length_ll_length_ll_f] .
+    using hfref_compI_PRE_aux[OF length_aa_u_hnr length_ll_length_ll_f] .
 
   have 1: \<open>?pre' = ?pre\<close>
     using ex_list_watched
     by (fastforce simp: comp_PRE_def prod_rel_def_internal relAPP_def map_fun_rel_def[abs_def]
-        p2rel_def lit_of_natP_def literal_of_neq_eq_nat_of_lit_eq_iff length_ll_def
+        p2rel_def lit_of_natP_def literal_of_neq_eq_nat_of_lit_eq_iff length_ll_def nat_lit_rel_def
         simp del: literal_of_nat.simps)
 
   have 2: \<open>?im' = ?im\<close>
     unfolding prod_hrp_comp by (auto simp: hrp_comp_def hr_comp_def)
   have 3: \<open>?f' = ?f\<close>
     by (auto simp: hrp_comp_def hr_comp_def)
-
+    
   show ?thesis
-    using H unfolding 1 2 3  .
+    using H unfolding 1 2 3 .
 qed
 
 
