Weidenbach_Book/WB_Word_Assn.thy
@@ -1,10 +1,10 @@
 theory WB_Word_Assn
 imports
-  CDCL_Two_Watched_Literals_List_Watched_Init_Code
   "$AFP/Word/Word"
+  IICF
 begin
 definition word_nat_rel :: "('a :: len0 Word.word \<times> nat) set" where
-  \<open>word_nat_rel = {(n, n'). unat n = n'}\<close>
+  \<open>word_nat_rel = br unat (\<lambda>_. True)\<close>
 
 abbreviation word_nat_assn :: "nat \<Rightarrow> 'a::len0 Word.word \<Rightarrow> assn" where
   \<open>word_nat_assn \<equiv> pure word_nat_rel\<close>
@@ -12,10 +12,10 @@ abbreviation word_nat_assn :: "nat \<Rightarrow> 'a::len0 Word.word \<Rightarrow
 lemma op_eq_word_nat:
   \<open>(uncurry (return oo (op = :: 'a :: len Word.word \<Rightarrow> _)), uncurry (RETURN oo op =)) \<in>
     word_nat_assn\<^sup>k *\<^sub>a word_nat_assn\<^sup>k \<rightarrow>\<^sub>a bool_assn\<close>
-  by sepref_to_hoare (sep_auto simp: word_nat_rel_def)
+  by sepref_to_hoare (sep_auto simp: word_nat_rel_def br_def)
 
 definition uint32_nat_rel :: "(uint32 \<times> nat) set" where
-  \<open>uint32_nat_rel = {(n, n'). nat_of_uint32 n = n'}\<close>
+  \<open>uint32_nat_rel = br nat_of_uint32 (\<lambda>_. True)\<close>
 
 abbreviation uint32_nat_assn :: "nat \<Rightarrow> uint32 \<Rightarrow> assn" where
   \<open>uint32_nat_assn \<equiv> pure uint32_nat_rel\<close>
@@ -26,12 +26,22 @@ lemma word_nat_of_uint32_Rep_inject[simp]: \<open>nat_of_uint32 ai = nat_of_uint
 lemma op_eq_uint32_nat:
   \<open>(uncurry (return oo (op = :: uint32 \<Rightarrow> _)), uncurry (RETURN oo op =)) \<in>
     uint32_nat_assn\<^sup>k *\<^sub>a uint32_nat_assn\<^sup>k \<rightarrow>\<^sub>a bool_assn\<close>
-  by sepref_to_hoare (sep_auto simp: uint32_nat_rel_def)
+  by sepref_to_hoare (sep_auto simp: uint32_nat_rel_def br_def)
 
 lemma unat_shiftr: \<open>unat (xi >> n) = unat xi div (2^n)\<close>
-  by (metis nat_int nat_shifl_div shiftr_div_2n shiftr_nat_def uint_nat)
+proof -
+  have [simp]: \<open>nat (2 * 2 ^ n) =  2 * 2 ^ n\<close> for n :: nat
+    by (metis nat_numeral nat_power_eq power_Suc rel_simps(27))
+  show ?thesis
+  unfolding unat_def
+  by (induction n arbitrary: xi)
+     (auto simp: shiftr_div_2n nat_div_distrib)
+qed
 
-lemma \<open>(return o (\<lambda>n. shiftr n 1), RETURN o shiftr1) \<in> word_nat_assn\<^sup>k \<rightarrow>\<^sub>a word_nat_assn\<close>
+instance uint32 :: heap
+  by standard (auto simp: inj_def exI[of _ nat_of_uint32])
+
+(* lemma \<open>(return o (\<lambda>n. shiftr n 1), RETURN o shiftr1) \<in> word_nat_assn\<^sup>k \<rightarrow>\<^sub>a word_nat_assn\<close>
   by sepref_to_hoare (sep_auto simp: shiftr1_def word_nat_rel_def unat_shiftr)
-
+ *)
 end
